Update proof to paper version

DeterminismTypes.v
@@ -2,24 +2,9 @@ Require Import Strings.String Lists.List Lists.ListSet PeanoNat EqNat Bool Funct
 Import ListNotations.
 
 (**
-NOTE: due to time constraints, the formalization is not yet fully updated
-to the paper. Should be updated by mid June. Differences are:
-- A different simplified Curry type system with only types Unit and Pairs.
-  Consequently, our expressions have different data constructors as well.
-- Compatibility is used differently, in the sense that we constructively
-  build compatible types and contexts, rather than using a
-  compatibility relation.
+NOTE: Formalization is now completely updated.
 
-For the reason that we still have to update the formalization,
-there are currently two small sections where this formalization
-is not yet completely machine-checked. We will address this in the near future.
-These points are the application of the substitution lemma on determinsm
-types in the preservation theorem for case and function application.
-At the moment, there is a consistency problem between the way compatibility
-is used in the preservation theorem statement and the way it is used in the
-substitution lemma.
-
-Other than these differences, you can check that this corresponds to the paper.
+You can check that this formalization corresponds to the paper.
 Just search in this document for the following important theorems and
 definitions:
 - "typeOf" corresponds to the simplified Curry type system
@@ -53,30 +38,25 @@ Section Types.
   Definition Arity := nat.
 
   Inductive TType : Type :=
-    | TUnit : TType
-    | TPair : TType -> TType -> TType
+    | TBool : TType
+    | TList : TType -> TType
     | TArrow : TType -> TType -> TType.
 
   Inductive Pattern : Type :=
-    | Pat : forall (n1 : nat) (t1 : TType) (n2 : nat) (t2 : TType)
+    | Pat : forall (n1 : nat) (t1 : TType) (n2 : nat)
           , n1 <> n2 -> Pattern.
 
   Inductive Exp : Type :=
-    | Var : nat -> Exp
-    | Unit : Exp
-    | Pair : Exp -> Exp -> Exp
-    | App : Exp -> Exp -> Exp
-    | Abs : nat -> TType -> Exp -> Exp
-    | Or  : Exp -> Exp -> Exp
-    | Case: Exp -> Branch -> Exp
-   with Branch : Type :=
-     | BranchUnit :            Exp -> Branch
-     | BranchPair : Pattern -> Exp -> Branch.
-
-  Scheme Exp_Branch_mut := Induction for Exp Sort Prop
-    with   Branch_Exp_mut := Induction for Branch Sort Prop.
-
-  Combined Scheme ExpBranch_mutind from Exp_Branch_mut, Branch_Exp_mut.
+    | Var    : nat -> Exp
+    | BTrue  : Exp
+    | BFalse : Exp
+    | Nil    : TType -> Exp
+    | Cons   : Exp -> Exp -> Exp
+    | App    : Exp -> Exp -> Exp
+    | Abs    : nat -> TType -> Exp -> Exp
+    | Or     : Exp -> Exp -> Exp
+    | CaseB  : Exp -> Exp -> Exp -> Exp
+    | CaseL  : Exp -> Exp -> Pattern -> Exp -> Exp.
 
   Definition notOr (e : Exp) : Prop :=
     match e with
@@ -86,9 +66,8 @@ Section Types.
 
   Fixpoint eqType (t1 t2 : TType) : bool :=
     match t1, t2 with
-    | TUnit, TUnit => true
-    | TPair t11 t12, TPair t21 t22 =>
-        andb (eqType t11 t21) (eqType t12 t22)
+    | TBool, TBool => true
+    | TList t1, TList t2 => eqType t1 t2
     | TArrow t11 t12, TArrow t21 t22 =>
         andb (eqType t11 t21) (eqType t12 t22)
     | _, _ => false
@@ -98,7 +77,7 @@ Section Types.
     eqType t t = true.
   Proof.
     induction t; simpl; try reflexivity.
-    - rewrite IHt1. rewrite IHt2. reflexivity.
+    - rewrite IHt. reflexivity.
     - rewrite IHt1. rewrite IHt2. reflexivity.
   Qed.
 
@@ -109,9 +88,7 @@ Section Types.
     - intros. generalize dependent t2. induction t1; intros.
       + destruct t2; try discriminate. reflexivity.
       + destruct t2; try discriminate. simpl in H.
-        apply Bool.andb_true_iff in H. destruct H.
-        apply IHt1_1 in H. apply IHt1_2 in H0.
-        subst. reflexivity.
+        apply IHt1 in H. subst. reflexivity.
       + destruct t2; try discriminate. simpl in H.
         apply Bool.andb_true_iff in H. destruct H.
         apply IHt1_1 in H. apply IHt1_2 in H0.
@@ -136,10 +113,18 @@ Section Types.
   Fixpoint typeOf (c : nat -> TType) (e : Exp) : option TType :=
     match e with
     | Var n => Some (c n)
-    | Unit => Some TUnit
-    | Pair e1 e2 => match (typeOf c e1), (typeOf c e2) with
-                    | Some t1, Some t2 => Some (TPair t1 t2)
-                    | _, _ => None
+    | BTrue => Some TBool
+    | BFalse => Some TBool
+    | Nil t => Some (TList t)
+    | Cons e1 e2 => match (typeOf c e2) with
+                    | Some t2 => match t2 with
+                      | TList t2' =>
+                        if eqTypeS (typeOf c e1) (Some t2')
+                        then Some (TList t2')
+                        else None
+                      | _ => None
+                      end
+                    | _ => None
                     end
     | App e1 e2 => match typeOf c e1, typeOf c e2 with
                    | Some (TArrow t1 t2), Some t1' =>
@@ -148,22 +133,28 @@ Section Types.
                    | _, _ => None
                    end
     | Abs n t e => match typeOf (update Nat.eqb c n t) e with
-                   | Some t' => Some (TArrow t t')
-                   | None => None
-                   end
+                  | Some t' => Some (TArrow t t')
+                  | None => None
+                  end
     | Or e1 e2 => let t1 := typeOf c e1 in if eqTypeS t1 (typeOf c e2)
                                           then t1 else None
-    | Case e1 brs => match brs, typeOf c e1 with
-                    | BranchUnit e2, Some TUnit => typeOf c e2
-                    | BranchPair (Pat n1 t1 n2 t2 H) e2,
-                      Some (TPair t1' t2') =>
-                        let c'  := update Nat.eqb c  n1 t1 in
-                        let c'' := update Nat.eqb c' n2 t2 in
-                        if eqType t1 t1' && eqType t2 t2'
-                          then typeOf c'' e2
-                          else None
+    | CaseB e1 e2 e3 => match typeOf c e1 with
+                  | Some TBool => match typeOf c e2, typeOf c e3 with
+                    | Some t1, Some t2 =>
+                      if eqType t1 t2 then Some t1 else None
                     | _, _ => None
                     end
+                  | _ => None
+                  end
+    | CaseL e1 e2 (Pat n1 t1' n2 _) e3 =>
+      if eqTypeS (typeOf c e1) (Some (TList t1'))
+        then if eqTypeS (typeOf c e2)
+                     (typeOf (update Nat.eqb
+                             (update Nat.eqb c n2 (TList t1'))
+                                n1 t1') e3)
+                then typeOf c e2
+                else None
+      else None
     end.
 
   Definition well_typed (c : nat -> TType) (e : Exp) : Prop :=
@@ -179,8 +170,8 @@ Section Types.
 
   Fixpoint compatible (d : DType) (t : TType) : Prop :=
     match d, t with
-    | D, TUnit => True
-    | D, TPair t1 t2 => True
+    | D, TBool => True
+    | D, TList _ => True
     | ND, _ => True
     | Arrow d1 d2, TArrow t1 t2 =>
         compatible d1 t1 /\ compatible d2 t2
@@ -189,22 +180,26 @@ Section Types.
 
   Fixpoint mkCompatible (t : TType) : DType :=
     match t with
-    | TUnit => D
-    | TPair t1 t2 => D
+    | TBool => D
+    | TList _ => D
     | TArrow t1 t2 => Arrow (mkCompatible t1) (mkCompatible t2)
     end.
 
   Lemma mkCompatible_compatible : forall t,
     compatible (mkCompatible t) t.
   Proof.
-    induction t; simpl; try constructor; auto.
+    induction t.
+    - reflexivity.
+    - reflexivity.
+    - simpl. split; [apply IHt1 | apply IHt2].
   Qed.
 
   Fixpoint beq_DType (d1 d2 : DType) : bool :=
     match d1, d2 with
     | D, D => true
     | ND, ND => true
-    | Arrow d1 d2, Arrow d1' d2' => andb (beq_DType d1 d1') (beq_DType d2 d2')
+    | Arrow d1 d2, Arrow d1' d2' =>
+      andb (beq_DType d1 d1') (beq_DType d2 d2')
     | _, _ => false
     end.
 
@@ -222,38 +217,36 @@ Section Context.
   Definition compatibleCtx (c : context) (cT : contextT) : Prop :=
     forall n, compatible (c n) (cT n).
 
-  Definition mkCompatibleCtx : contextT -> context :=
-    fun c => fun n =>  mkCompatible (c n).
+  Definition mkCompatibleCtx (cT : contextT) : context :=
+    fun n => mkCompatible (cT n).
 
   Lemma update_compatible :
-    forall Gamma Rho n t,
-    Gamma = mkCompatibleCtx Rho ->
-    update Nat.eqb Gamma n (mkCompatible t) =
-    mkCompatibleCtx (update Nat.eqb Rho n t).
+    forall Gamma Rho n t d,
+    compatibleCtx Gamma Rho ->
+    compatible d t ->
+    compatibleCtx (update Nat.eqb Gamma n d)
+                  (update Nat.eqb Rho n t).
   Proof.
-    intros. apply functional_extensionality. intro x.
-    unfold mkCompatibleCtx. unfold update.
-    destruct (Nat.eqb n x) eqn:Heq.
-    - reflexivity.
-    - unfold mkCompatibleCtx in H. rewrite H. reflexivity.
+    intros. unfold compatibleCtx. intro n0.
+    unfold update. destruct (Nat.eqb n n0) eqn:Heq.
+    - assumption.
+    - unfold compatibleCtx in H. apply H.
   Qed.
 
   Lemma update_update_compatible :
-    forall Gamma Rho n1 n2 t1 t2,
-    Gamma = mkCompatibleCtx Rho ->
-    let Gamma' := update Nat.eqb Gamma n1 (mkCompatible t1) in
-    update Nat.eqb Gamma' n2 (mkCompatible t2) =
-    mkCompatibleCtx (update Nat.eqb (update Nat.eqb Rho n1 t1) n2 t2).
+    forall Gamma Rho n1 n2 t1 d1 t2 d2,
+    compatibleCtx Gamma Rho ->
+    compatible d1 t1 ->
+    compatible d2 t2 ->
+    let Gamma' := update Nat.eqb Gamma n1 d1 in
+    compatibleCtx (update Nat.eqb Gamma' n2 d2)
+                  (update Nat.eqb (update Nat.eqb Rho n1 t1) n2 t2).
   Proof.
-    intros. apply functional_extensionality. intro x.
-    unfold mkCompatibleCtx. unfold update.
-    destruct (Nat.eqb n1 x) eqn:Heq1;
-    destruct (Nat.eqb n2 x) eqn:Heq2; try reflexivity.
-    - subst Gamma'. unfold update.
-      rewrite Heq1. reflexivity.
-    - subst Gamma'. unfold update.
-      rewrite Heq1. unfold mkCompatibleCtx in H.
-      rewrite H. reflexivity.
+    intros. unfold compatibleCtx in *. intro n0.
+    subst Gamma'. unfold update in *.
+    destruct (Nat.eqb n1 n0) eqn:Heq1;
+    destruct (Nat.eqb n2 n0) eqn:Heq2; try assumption.
+    - apply H.
   Qed.
 
 End Context.
@@ -398,28 +391,162 @@ End Subtyping.
    connecting the operational behavior with static determinism properties. *)
 Section DetTyping.
 
-  Fixpoint d_fun (n : Arity) : DType :=
-    match n with
-    | 0 => D
-    | S m => Arrow D (d_fun m)
-    end.
+  Definition lub2 (d1 d2 : DType) : DType :=
+    if more_specific d1 d2 then d2
+    else if more_specific d2 d1 then d1
+    else ND.
+
+  Definition lub (d1 d2 d3 : DType) : DType :=
+    lub2 (lub2 d1 d2) d3.
+
+  Lemma compatible_lub : forall d1 d2 d3 t,
+    compatible d1 TBool ->
+    compatible d2 t ->
+    compatible d3 t ->
+    compatible (lub d1 d2 d3) t.
+  Proof.
+    intros d1 d2 d3 t Hc1 Hc2 Hc3.
+    unfold lub. unfold lub2.
+    destruct (more_specific d1 d2) eqn:H1.
+    - destruct (more_specific d2 d3) eqn:H2.
+      + assumption.
+      + destruct (more_specific d3 d2) eqn:H3.
+        * assumption.
+        * reflexivity.
+    - destruct (more_specific d2 d1) eqn:H4.
+      + destruct (more_specific d1 d3) eqn:H5.
+        * assumption.
+        * destruct (more_specific d3 d1) eqn:H6.
+          -- destruct d1; inversion Hc1.
+             ++  destruct t; try reflexivity.
+                 destruct d2; inversion Hc2;
+                 inversion H4.
+             ++ reflexivity.
+          -- reflexivity.
+      + simpl. destruct d3; auto; reflexivity.
+  Qed.
+
+  (* Lemma compatible_lub_r : forall d1 d2 d3 t,
+    compatible (lub d1 d2 d3) t ->
+    compatible d2 t.
+  Proof.
+    intros. unfold lub in H. unfold lub2 in H.
+    destruct (more_specific d1 d2) eqn:H1.
+    - destruct (more_specific d2 d3) eqn:H2.
+      + destruct d2, d3, t; try discriminate;
+        try reflexivity;
+        inversion H. reflexivity.
+      + destruct (more_specific d3 d2) eqn:H3.
+        * assumption.
+        * inversion H. reflexivity. *)
+
+  Lemma more_specific_lub2: forall d1 d2 x1 x2,
+    compatible d1 TBool ->
+    more_specific d1 x1 = true ->
+    more_specific d2 x2 = true ->
+    more_specific (lub2 d1 d2) (lub2 x1 x2) = true.
+  Proof.
+    intros d1 d2 x1 x2 C1 H1 H2.
+    unfold lub2. destruct (more_specific d1 d2) eqn:H3.
+    - destruct (more_specific x1 x2) eqn:H4.
+      + assumption.
+      + destruct (more_specific x2 x1) eqn:H5.
+        * eapply more_specific_transitive.
+          apply H2. apply H5.
+        * apply more_specific_ND.
+    - destruct (more_specific d2 d1) eqn:H5.
+      + destruct (more_specific x1 x2) eqn:H6.
+        * eapply more_specific_transitive.
+          apply H1. apply H6.
+        * destruct (more_specific x2 x1) eqn:H7.
+          -- assumption.
+          -- apply more_specific_ND.
+      + destruct (more_specific x1 x2) eqn:H6.
+        * destruct d1, d2, x1, x2;
+          try discriminate;
+          try reflexivity.
+          inversion C1.
+        * destruct (more_specific x2 x1) eqn:H7.
+          --  destruct d1, d2, x1, x2;
+              try discriminate;
+              try reflexivity.
+              inversion C1.
+          -- reflexivity.
+  Qed.
+
+  Lemma more_specific_lub: forall x1 x2 x3 d1 d2 d3,
+    compatible x1 TBool ->
+    more_specific x1 d1 = true ->
+    more_specific x2 d2 = true ->
+    more_specific x3 d3 = true ->
+    more_specific (lub x1 x2 x3) (lub d1 d2 d3) = true.
+  Proof.
+    intros x1 x2 x3 d1 d2 d3 C1 H1 H2 H3.
+    unfold lub.
+    apply more_specific_lub2; try assumption.
+    - destruct x1, x2; try discriminate;
+      try reflexivity.
+      inversion C1.
+    - apply more_specific_lub2; try assumption.
+  Qed.
+
+  Lemma more_specific_lub' : forall d1 d2 d3,
+    more_specific d2 (lub d1 d2 d3) = true.
+  Proof.
+    intros. unfold lub, lub2.
+    destruct (more_specific d1 d2) eqn:H1.
+    - destruct (more_specific d2 d3) eqn:H2.
+      + assumption.
+      + destruct (more_specific d3 d2) eqn:H3.
+        * apply more_specific_refl.
+        * apply more_specific_ND.
+    - destruct (more_specific d2 d1) eqn:H4.
+      + destruct (more_specific d1 d3) eqn:H5.
+        * eapply more_specific_transitive; eassumption.
+        * destruct (more_specific d3 d1) eqn:H6.
+          -- assumption.
+          -- apply more_specific_ND.
+      + simpl. destruct d3; simpl; apply more_specific_ND.
+  Qed.
+
+  Lemma more_specific_lub'' : forall d1 d2 d3,
+    more_specific d3 (lub d1 d2 d3) = true.
+  Proof.
+    intros. unfold lub, lub2.
+    destruct (more_specific d1 d2) eqn:H1.
+    - destruct (more_specific d2 d3) eqn:H2.
+      + apply more_specific_refl.
+      + destruct (more_specific d3 d2) eqn:H3.
+        * assumption.
+        * apply more_specific_ND.
+    - destruct (more_specific d2 d1) eqn:H4.
+      + destruct (more_specific d1 d3) eqn:H5.
+        * apply more_specific_refl.
+        * destruct (more_specific d3 d1) eqn:H6.
+          -- assumption.
+          -- apply more_specific_ND.
+      + simpl. destruct d3; reflexivity.
+  Qed.
 
   Reserved Notation "Gamma '|-' e ':::' delta" (at level 40).
   Inductive hasDType : context -> Exp -> DType -> Prop :=
     | Rule_Var : forall Gamma x d,
           (Gamma x) = d ->
           Gamma |- Var x ::: d
-    | Rule_Unit : forall Gamma d,
-          d = d_fun 0 ->
-          Gamma |- Unit ::: d
-    | Rule_Pair : forall Gamma e1 e2 d1 d2 d3,
+    | Rule_BTrue : forall Gamma,
+          Gamma |- BTrue ::: D
+    | Rule_BFalse : forall Gamma,
+          Gamma |- BFalse ::: D
+    | Rule_Nil : forall Gamma t,
+          Gamma |- Nil t ::: D
+    | Rule_Cons : forall Gamma e1 e2 d1 d2 d3,
           Gamma |- e1 ::: d1 ->
           Gamma |- e2 ::: d2 ->
           d3 = match d1, d2 with
               | D, D => D
               | _, _ => ND
               end ->
-          Gamma |- Pair e1 e2 ::: d3
+          Gamma |- Cons e1 e2 ::: d3
     | Rule_AppND : forall Gamma e1 e2 d1 d2,
           Gamma |- e1 ::: d1 ->
           Gamma |- e2 ::: d2 ->
@@ -429,37 +556,31 @@ Section DetTyping.
           Gamma |- e2 ::: d3 ->
           d4 = decide d1 d3 d2 ->
           Gamma |- App e1 e2 ::: d4
-    | Rule_Abs : forall Gamma x e d1 d2 t,
-          d1 = mkCompatible t ->
+    | Rule_Abs : forall Gamma x e d1 d2 t1,
+          compatible d1 t1 ->
           let Gamma' := update Nat.eqb Gamma x d1 in
           Gamma' |- e ::: d2 ->
-          Gamma |- Abs x t e ::: Arrow d1 d2
+          Gamma |- Abs x t1 e ::: Arrow d1 d2
     | Rule_Choice : forall Gamma e1 e2 d1 d2,
           Gamma |- e1 ::: d1 ->
           Gamma |- e2 ::: d2 ->
           Gamma |- Or e1 e2 ::: ND
-    | Rule_CaseNDUnit : forall Gamma e1 e2 d,
-          Gamma |- e1 ::: ND ->
-          Gamma |- e2 ::: d ->
-          Gamma |- Case e1 (BranchUnit e2) ::: ND
-    | Rule_CaseNDPair : forall Gamma e1 e2 n1 n2 t1 t2 d H,
-          Gamma |- e1 ::: ND ->
-          let Gamma'  := update Nat.eqb Gamma  n1 (mkCompatible t1) in
-          let Gamma'' := update Nat.eqb Gamma' n2 (mkCompatible t2) in
-          Gamma'' |- e2 ::: d ->
-          let p := Pat n1 t1 n2 t2 H in
-          Gamma |- Case e1 (BranchPair p e2) ::: ND
-    | Rule_CaseDUnit : forall Gamma e1 e2 d,
-          Gamma |- e1 ::: D ->
-          Gamma |- e2 ::: d ->
-          Gamma |- Case e1 (BranchUnit e2) ::: d
-    | Rule_CaseDPair : forall Gamma e1 e2 n1 n2 t1 t2 d H,
-          Gamma |- e1 ::: D ->
-          let Gamma'  := update Nat.eqb Gamma  n1 (mkCompatible t1) in
-          let Gamma'' := update Nat.eqb Gamma' n2 (mkCompatible t2) in
-          Gamma'' |- e2 ::: d ->
-          let p := Pat n1 t1 n2 t2 H in
-          Gamma |- Case e1 (BranchPair p e2) ::: d
+    | Rule_CaseBool : forall Gamma e1 e2 e3 d1 d2 d3,
+          Gamma |- e1 ::: d1 ->
+          Gamma |- e2 ::: d2 ->
+          Gamma |- e3 ::: d3 ->
+          Gamma |- CaseB e1 e2 e3 ::: lub d1 d2 d3
+    | Rule_CaseList :
+        forall Gamma e1 e2 e3 n1 n2 d1 t1 d2 d_1 d_2 d_3 H,
+          Gamma |- e1 ::: d_1 ->
+          compatible d1 t1 ->
+          compatible d2 (TList t1) ->
+          Gamma |- e2 ::: d_2 ->
+          let Gamma'  := update Nat.eqb Gamma  n1 d1 in
+          let Gamma'' := update Nat.eqb Gamma' n2 d2 in
+          Gamma'' |- e3 ::: d_3 ->
+          let p := Pat n1 t1 n2 H in
+          Gamma |- CaseL e1 e2 p e3 ::: lub d_1 d_2 d_3
     where "Gamma '|-' e ':::' delta" := (hasDType Gamma e delta).
 
 End DetTyping.
@@ -472,22 +593,23 @@ Section SmallStepSemantics.
   Fixpoint subst (n : nat) (v : Exp) (e : Exp) : Exp :=
     match e with
     | Var x => if Nat.eqb x n then v else e
-    | Unit => Unit
-    | Pair e1 e2 => Pair (subst n v e1) (subst n v e2)
+    | BTrue => BTrue
+    | BFalse => BFalse
+    | Nil t => Nil t
+    | Cons e1 e2 => Cons (subst n v e1) (subst n v e2)
     | App e1 e2 => App (subst n v e1) (subst n v e2)
     | Abs x t e => if Nat.eqb x n
                     then Abs x t e
                     else Abs x t (subst n v e)
     | Or e1 e2 => Or (subst n v e1) (subst n v e2)
-    | Case e br => Case (subst n v e)
-      (match br with
-        | BranchUnit e2 =>
-            BranchUnit (subst n v e2)
-        | BranchPair (Pat n1 t1 n2 t2 H) e2 =>
-            if Nat.eqb n n1 || Nat.eqb n n2
-              then BranchPair (Pat n1 t1 n2 t2 H) e2
-              else BranchPair (Pat n1 t1 n2 t2 H) (subst n v e2)
-        end)
+    | CaseB e1 e2 e3 =>
+        CaseB (subst n v e1) (subst n v e2) (subst n v e3)
+    | CaseL e1 e2 (Pat n1 t1 n2 H) e3 =>
+      if Nat.eqb n n1 || Nat.eqb n n2
+        then CaseL (subst n v e1) (subst n v e2)
+                   (Pat n1 t1 n2 H) e3
+        else CaseL (subst n v e1) (subst n v e2)
+          (Pat n1 t1 n2 H) (subst n v e3)
     end.
 
   Fixpoint subst_all (ns : list (nat * Exp * TType)) (e : Exp) : Exp :=
@@ -505,36 +627,35 @@ Section SmallStepSemantics.
   Fixpoint freeVars (e : Exp) : list nat :=
     match e with
     | Var x => [x]
-    | Unit => []
-    | Pair e1 e2 => freeVars e1 ++ freeVars e2
+    | BTrue => []
+    | BFalse => []
+    | Nil _ => []
+    | Cons e1 e2 => freeVars e1 ++ freeVars e2
     | App e1 e2 => freeVars e1 ++ freeVars e2
     | Abs x _ e' => removeb Nat.eqb x (freeVars e')
     | Or e1 e2 => freeVars e1 ++ freeVars e2
-    | Case e' br =>
-        let vars := freeVars e' in
-        match br with
-        | BranchUnit e'' => vars ++ freeVars e''
-        | BranchPair (Pat n1 _ n2 _ _) e'' =>
-            vars ++ removeb Nat.eqb n1
-                    (removeb Nat.eqb n2 (freeVars e''))
-        end
+    | CaseB e1 e2 e3 =>
+        freeVars e1 ++ freeVars e2 ++ freeVars e3
+    | CaseL e1 e2 (Pat n1 _ n2 _) e3 =>
+        freeVars e1 ++ freeVars e2 ++
+        removeb Nat.eqb n1 (removeb Nat.eqb n2 (freeVars e3))
     end.
 
   Fixpoint boundVars (e : Exp) : list nat :=
     match e with
     | Var _ => []
-    | Unit => []
-    | Pair e1 e2 => boundVars e1 ++ boundVars e2
+    | BTrue => []
+    | BFalse => []
+    | Nil _ => []
+    | Cons e1 e2 => boundVars e1 ++ boundVars e2
     | App e1 e2 => boundVars e1 ++ boundVars e2
     | Abs x _ e' => x :: boundVars e'
     | Or e1 e2 => boundVars e1 ++ boundVars e2
-    | Case e' br =>
-        let vars := boundVars e' in
-        match br with
-        | BranchUnit e'' => vars ++ boundVars e''
-        | BranchPair (Pat n1 _ n2 _ _) e'' => vars ++
-            n1 :: n2 :: boundVars e''
-        end
+    | CaseB e1 e2 e3 =>
+        boundVars e1 ++ boundVars e2 ++ boundVars e3
+    | CaseL e1 e2 (Pat n1 _ n2 _) e3 =>
+        boundVars e1 ++ boundVars e2 ++
+        n1 :: n2 :: boundVars e3
     end.
 
   Fixpoint anyIn (xs ys : list nat) : bool :=
@@ -557,16 +678,21 @@ Section SmallStepSemantics.
                     | None => None
                     | Some e1' => Some (App e1' e2)
                     end
-    | Case (Or e1 e2) br =>
-        Some (Or (Case e1 br) (Case e2 br))
-    | Case Unit (BranchUnit e) => Some e
-    | Case (Pair e1 e2)
-        (BranchPair (Pat n1 t1 n2 t2 _) e3) =>
-          if anyIn (freeVars (Pair e1 e2)) (n1::n2::boundVars e3)
+    | CaseB (Or e1 e2) e3 e4 =>
+        Some (Or (CaseB e1 e3 e4) (CaseB e2 e3 e4))
+    | CaseL (Or e1 e2) e3 (Pat n1 t1 n2 H) e4 =>
+        Some (Or (CaseL e1 e3 (Pat n1 t1 n2 H) e4)
+                 (CaseL e2 e3 (Pat n1 t1 n2 H) e4))
+    | CaseB BFalse e2 e3 => Some e2
+    | CaseB BTrue e2 e3 => Some e3
+    | CaseL (Nil _) e2 _ e3 => Some e2
+    | CaseL (Cons e1 e2) e3 (Pat n1 t1 n2 H) e4 =>
+          if anyIn (freeVars (Cons e1 e2)) (n1::n2::boundVars e4)
             then None
             else if anyIn (freeVars e2) (boundVars e1)
               then None
-              else Some (subst_all [(n1, e1, t1); (n2, e2, t2)] e3)
+              else Some (subst_all [(n1, e1, t1);
+                                    (n2, e2, TList t1)] e4)
     | Or e1 e2 => match step e1 with
                   | None => match step e2 with
                             | None => None
@@ -574,12 +700,12 @@ Section SmallStepSemantics.
                             end
                   | Some e1' => Some (Or e1' e2)
                   end
-    | Pair e1 e2 => match step e1 with
+    | Cons e1 e2 => match step e1 with
                     | None => match step e2 with
                               | None => None
-                              | Some e2' => Some (Pair e1 e2')
+                              | Some e2' => Some (Cons e1 e2')
                               end
-                    | Some e1' => Some (Pair e1' e2)
+                    | Some e1' => Some (Cons e1' e2)
                     end
     | _ => None
     end.
@@ -623,12 +749,12 @@ Section Examples.
       reflexivity.
   Qed.
 
-  Example exCons : Gamma1 |- Unit ::: D.
+  Example exCons : Gamma1 |- Nil TBool ::: D.
   Proof.
-      apply Rule_Unit; trivial.
+      apply Rule_Nil; trivial.
   Qed.
 
-  Example exApp : Gamma1 |- App (Abs 2 TUnit (Var 2)) (Var 1) ::: D.
+  Example exApp : Gamma1 |- App (Abs 2 TBool (Var 2)) (Var 1) ::: D.
   Proof.
       eapply Rule_AppFun with (d1 := D) (d2 := D) (d3 := D).
       + apply Rule_Abs. reflexivity.
@@ -638,12 +764,12 @@ Section Examples.
       + reflexivity.
   Qed.
 
-  Example exAppEval : App (Abs 2 TUnit (Var 2)) (Var 1) ==>* Var 1.
+  Example exAppEval : App (Abs 2 TBool (Var 2)) (Var 1) ==>* Var 1.
   Proof.
       eapply Multi_Step_Many. apply Single_Step. reflexivity. apply Multi_Step_Refl.
   Qed.
 
-  Example exAbs : Gamma1 |- Abs 2 TUnit (Var 1) ::: Arrow D D.
+  Example exAbs : Gamma1 |- Abs 2 TBool (Var 1) ::: Arrow D D.
   Proof.
       apply Rule_Abs. reflexivity.
       apply Rule_Var. reflexivity.
@@ -651,7 +777,7 @@ Section Examples.
 
   Definition Gamma2 := update Nat.eqb (fun _ => ND) 1 (Arrow (Arrow D D) (Arrow D D)).
 
-  Example exPoly : Gamma2 |- App (Var 1) (Abs 2 TUnit (Var 2)) ::: Arrow D D.
+  Example exPoly : Gamma2 |- App (Var 1) (Abs 2 TBool (Var 2)) ::: Arrow D D.
   Proof.
       eapply Rule_AppFun with (d1 := Arrow D D) (d2 := Arrow D D) (d3 := Arrow D D).
       + apply Rule_Var. reflexivity.
@@ -667,20 +793,13 @@ Section Examples.
       - apply Rule_Var. reflexivity.
   Qed.
 
-  Example exCase : Gamma1 |- Case (Var 42) (BranchUnit (Var 1)) ::: ND.
-  Proof.
-      eapply Rule_CaseNDUnit.
-      apply Rule_Var. reflexivity.
-      apply Rule_Var. reflexivity.
-  Qed.
-
   (*
   1 = allValues :? Any -> Det
   2 = \x -> id x ? not x :? Any -> Any
   result must not be of type D
   *)
-  Definition RhoAV' := update Nat.eqb (fun _ => TUnit) 1 (TArrow TUnit TUnit).
-  Definition RhoAV  := update Nat.eqb RhoAV' 2 (TArrow TUnit TUnit).
+  Definition RhoAV' := update Nat.eqb (fun _ => TBool) 1 (TArrow TBool TBool).
+  Definition RhoAV  := update Nat.eqb RhoAV' 2 (TArrow TBool TBool).
   Definition GammaAV := mkCompatibleCtx RhoAV.
   Example exAllValues : GammaAV |- App (Var 1) (Var 2) ::: ND.
   Proof.
@@ -705,29 +824,29 @@ Section Examples.
   (not ? id) :? Any
   (not ? id) True :? Any
   *)
-  Definition RhoC' := update Nat.eqb (fun _ => TUnit) 1 (TArrow TUnit TUnit).
-  Definition RhoC  := update Nat.eqb RhoC' 2 (TArrow TUnit TUnit).
+  Definition RhoC' := update Nat.eqb (fun _ => TBool) 1 (TArrow TBool TBool).
+  Definition RhoC  := update Nat.eqb RhoC' 2 (TArrow TBool TBool).
   Definition GammaC := mkCompatibleCtx RhoC.
-  Example exChoice2 : GammaC |- App (Or (Var 1) (Var 2)) Unit ::: ND.
+  Example exChoice2 : GammaC |- App (Or (Var 1) (Var 2)) BFalse ::: ND.
   Proof.
       eapply Rule_AppND.
       - eapply Rule_Choice.
         + apply Rule_Var. reflexivity.
         + apply Rule_Var. reflexivity.
-      - apply Rule_Unit. reflexivity.
+      - apply Rule_BFalse.
   Qed.
   Lemma exChoice2_must_use_AppND :
-  forall d,
-    GammaC |- App (Or (Var 1) (Var 2)) Unit ::: d ->
+  forall b d,
+    GammaC |- App (Or (Var 1) (Var 2)) b ::: d ->
     d = ND /\
     (forall d1 d2,
-      ~ (GammaC |- Or (Var 1) (Var 2) ::: d1 /\ GammaC |- Unit ::: d2 /\
+      ~ (GammaC |- Or (Var 1) (Var 2) ::: d1 /\ GammaC |- b ::: d2 /\
          exists d3 d4 d5,
            GammaC |- Or (Var 1) (Var 2) ::: Arrow d3 d4 /\
-           GammaC |- Unit ::: d5 /\
+           GammaC |- b ::: d5 /\
            d = decide d3 d5 d4)).
   Proof.
-    intros d H.
+    intros b d H.
     inversion H; subst.
     - split; auto.
       intros d3 d4 [H1 [H2 [d5 [d6 [d7 [H4 [H6 H7]]]]]]].
@@ -742,15 +861,17 @@ End Examples.
    relationship between expression structure and type safety. *)
 Section WellTypedness.
 
-  Lemma well_typed_Pair :
+  Lemma well_typed_Cons :
     forall Rho e1 e2,
-    well_typed Rho (Pair e1 e2) ->
+    well_typed Rho (Cons e1 e2) ->
     well_typed Rho e1 /\ well_typed Rho e2.
   Proof.
     intros. unfold well_typed in *.
     unfold typeOf in H. fold typeOf in H.
-    destruct (typeOf Rho e1) eqn:Heq1;
     destruct (typeOf Rho e2) eqn:Heq2;
+    try inversion H; subst.
+    destruct t; try inversion H; subst.
+    destruct (typeOf Rho e1) eqn:Heq1;
     auto.
   Qed.
 
@@ -787,53 +908,19 @@ Section WellTypedness.
     destruct (typeOf Rho e2) eqn:Heq2; auto.
   Qed.
 
-  Lemma well_typed_Case_Unit :
-    forall Rho e brs,
-    well_typed Rho (Case e (BranchUnit brs)) ->
-    well_typed Rho e /\ well_typed Rho brs.
+  Lemma well_typed_CaseB :
+    forall Rho e1 e2 e3,
+    well_typed Rho (CaseB e1 e2 e3) ->
+    well_typed Rho e1 /\ well_typed Rho e2 /\ well_typed Rho e3.
   Proof.
     intros. unfold well_typed in *.
     unfold typeOf in H. fold typeOf in H.
-    destruct (typeOf Rho e) eqn:Heq1;
-    destruct (typeOf Rho brs) eqn:Heq2; auto.
+    destruct (typeOf Rho e1) eqn:Heq1;
+    destruct (typeOf Rho e2) eqn:Heq2;
+    destruct (typeOf Rho e3) eqn:Heq3; auto;
     destruct t; auto.
   Qed.
 
-  Lemma well_typed_Case_Pair :
-    forall Rho e n1 n2 t1 t2 brs HU,
-    well_typed Rho (Case e (BranchPair (Pat n1 t1 n2 t2 HU) brs)) ->
-    let Rho'  := update Nat.eqb Rho  n1 t1 in
-    let Rho'' := update Nat.eqb Rho' n2 t2 in
-    well_typed Rho e /\ well_typed Rho'' brs.
-  Proof.
-    intros. unfold well_typed in *.
-    unfold typeOf in H. fold typeOf in H.
-    destruct (typeOf Rho e) eqn:Heq1;
-    destruct (typeOf Rho'' brs) eqn:Heq2; auto.
-    destruct t; auto.
-    subst Rho''. subst Rho'.
-    destruct (eqType t1 t3 && eqType t2 t4).
-    rewrite Heq2 in H. auto. auto.
-  Qed.
-
-  Lemma well_typed_Case :
-    forall Rho e b,
-    well_typed Rho (Case e b) ->
-    well_typed Rho e.
-  Proof.
-    intros. unfold well_typed in *.
-    unfold typeOf in H. fold typeOf in H.
-    destruct (typeOf Rho e) eqn:Heq1; auto.
-    destruct b; auto; destruct p; auto.
-  Qed.
-
-End WellTypedness.
-
-(* Section PreservationTTypesHelper:
-   Helper lemmas for the preservation theorem, primarily focused on
-   variable management, substitution properties, and interaction between
-   free and bound variables. *)
-Section PreservationTTypesHelper.
 
   Lemma double_update_indep :
     forall {V : Type} (Rho : nat -> V) n1 t1 n2 t2,
@@ -859,6 +946,41 @@ Section PreservationTTypesHelper.
     unfold update.
     destruct (Nat.eqb n1 x); try reflexivity.
   Qed.
+
+  Lemma well_typed_CaseL :
+    forall Rho e1 e2 e3 n1 t1 n2 HU,
+    well_typed Rho (CaseL e1 e2 (Pat n1 t1 n2 HU) e3) ->
+    let Rho'  := update Nat.eqb Rho  n1 t1 in
+    let Rho'' := update Nat.eqb Rho' n2 (TList t1) in
+    well_typed Rho e1 /\ well_typed Rho e2 /\ well_typed Rho'' e3.
+  Proof.
+    intros. unfold well_typed in *.
+    unfold typeOf in H. fold typeOf in H.
+    destruct (typeOf Rho e1) eqn:Heq1;
+    try inversion H; simpl in H;
+    destruct (eqType t (TList t1)) eqn:Heq;
+    try inversion H. apply eq_Type_eq in Heq. subst.
+    destruct (typeOf Rho e2) eqn:Heq2;
+    try inversion H; simpl in H;
+    destruct (typeOf (update Nat.eqb
+                     (update Nat.eqb Rho n2 (TList t1))
+                      n1 t1) e3) eqn:Heq3;
+    try inversion H; simpl in H.
+    destruct (eqType t t0) eqn:Heq4;
+    try inversion H; simpl in H.
+    apply eq_Type_eq in Heq4. subst.
+    subst Rho'. subst Rho''.
+    rewrite double_update_indep.
+    rewrite Heq3. auto. assumption.
+  Qed.
+
+End WellTypedness.
+
+(* Section PreservationTTypesHelper:
+   Helper lemmas for the preservation theorem, primarily focused on
+   variable management, substitution properties, and interaction between
+   free and bound variables. *)
+Section PreservationTTypesHelper.
 
   Lemma existsb_concat :
     forall (l1 l2 : list nat) (beq : nat -> nat -> bool) x,
@@ -977,9 +1099,9 @@ Section PreservationTTypesHelper.
         * apply IHe1; assumption.
   Qed.
 
-  Lemma anyIn_Pair :
+  Lemma anyIn_Cons :
     forall e1_1 e1_2 e2,
-    anyIn (freeVars e2) (boundVars (Pair e1_1 e1_2)) = false ->
+    anyIn (freeVars e2) (boundVars (Cons e1_1 e1_2)) = false ->
     anyIn (freeVars e2) (boundVars e1_1) = false /\
     anyIn (freeVars e2) (boundVars e1_2) = false.
   Proof.
@@ -990,7 +1112,7 @@ Section PreservationTTypesHelper.
 
   Lemma anyIn_Pair2 :
     forall e1_1 e1_2 e2,
-    anyIn (freeVars (Pair e1_1 e1_2)) (boundVars e2) = false ->
+    anyIn (freeVars (Cons e1_1 e1_2)) (boundVars e2) = false ->
     anyIn (freeVars e1_1) (boundVars e2) = false /\
     anyIn (freeVars e1_2) (boundVars e2) = false.
   Proof.
@@ -1032,27 +1154,33 @@ Section PreservationTTypesHelper.
     apply anyIn_concat1 in H. assumption.
   Qed.
 
-  Lemma anyIn_Case_Unit :
-    forall e e1 e2,
-    anyIn (freeVars e) (boundVars (Case e1 (BranchUnit e2))) = false ->
+  Lemma anyIn_Case_Bool :
+    forall e e1 e2 e3,
+    anyIn (freeVars e) (boundVars (CaseB e1 e2 e3)) = false ->
     anyIn (freeVars e) (boundVars e1) = false /\
-    anyIn (freeVars e) (boundVars e2) = false.
+    anyIn (freeVars e) (boundVars e2) = false /\
+    anyIn (freeVars e) (boundVars e3) = false.
   Proof.
-    intros e e1 e2 H.
+    intros e e1 e2 e3 H.
     unfold boundVars in H. fold boundVars in H.
-    apply anyIn_concat1 in H. assumption.
+    apply anyIn_concat1 in H. destruct H.
+    apply anyIn_concat1 in H0.
+    split; assumption.
   Qed.
 
-  Lemma anyIn_Case_Pair :
-    forall e e1 n1 t1 n2 t2 e2 HU,
-    anyIn (freeVars e) (boundVars (Case e1
-      (BranchPair (Pat n1 t1 n2 t2 HU) e2))) = false ->
+  Lemma anyIn_Case_List :
+    forall e e1 n1 t1 n2 e2 e3 HU,
+    anyIn (freeVars e) (boundVars (CaseL e1
+      e2 (Pat n1 t1 n2 HU) e3)) = false ->
     anyIn (freeVars e) (boundVars e1) = false /\
-    anyIn (freeVars e) (n1 :: n2 :: boundVars e2) = false.
+    anyIn (freeVars e) (boundVars e2) = false /\
+    anyIn (freeVars e) (n1 :: n2 :: boundVars e3) = false.
   Proof.
-    intros e e1 n1 t1 n2 t2 e2 HU H.
+    intros e e1 n1 t1 n2 e2 e3 HU H.
     unfold boundVars in H. fold boundVars in H.
-    apply anyIn_concat1 in H. assumption.
+    apply anyIn_concat1 in H. destruct H.
+    apply anyIn_concat1 in H0.
+    split; assumption.
   Qed.
 
   Lemma anyIn_removeb : forall xs n n1,
@@ -1079,18 +1207,22 @@ Section PreservationTTypesHelper.
     anyIn (freeVars e) [n] = false ->
     typeOf (update Nat.eqb Rho n t2) e = typeOf Rho e.
   Proof.
-    fix typeOf_unbound 1.
-    --
     induction e; intros Rho n1 t1 t2 H H1; simpl in *.
     - destruct (Nat.eqb n n1) eqn:Heq; inversion H1.
       unfold update. rewrite Nat.eqb_sym in Heq. rewrite Heq.
       reflexivity.
     - reflexivity.
-    - destruct (typeOf Rho e1) eqn:Heq1,
-               (typeOf Rho e2) eqn:Heq2; try discriminate.
-      inversion H. subst. eapply anyIn_concat2 in H1.
+    - reflexivity.
+    - reflexivity.
+    - destruct (typeOf Rho e2) eqn:Heq2; try discriminate.
+      destruct t; try discriminate.
+      destruct (typeOf Rho e1) eqn:Heq1; try discriminate.
+      simpl in H. destruct (eqType t0 t) eqn:Heq3; try discriminate.
+      apply eq_Type_eq in Heq3. inversion H. subst. simpl.
+      rewrite eqType_refl. eapply anyIn_concat2 in H1.
       destruct H1 as [H1 H2]. erewrite IHe1. erewrite IHe2.
-      rewrite Heq1. rewrite Heq2. reflexivity. apply Heq2.
+      rewrite Heq1. rewrite Heq2. rewrite eqTypeS_refl.
+      reflexivity. apply Heq2.
       assumption. apply Heq1. assumption.
     - destruct (typeOf Rho e1) eqn:Heq1,
                (typeOf Rho e2) eqn:Heq2; try discriminate;
@@ -1118,39 +1250,55 @@ Section PreservationTTypesHelper.
       destruct H1 as [H1 H2]. erewrite IHe1. erewrite IHe2.
       rewrite Heq1. rewrite Heq2. rewrite eqTypeS_refl.
       reflexivity. apply Heq2. assumption. apply Heq1. assumption.
-    - destruct b.
-      + destruct (typeOf Rho e) eqn:Heq1; try discriminate.
-        destruct t; try discriminate.
-        inversion H. subst. eapply anyIn_concat2 in H1.
-        destruct H1 as [H3 H4]. erewrite IHe.
-        rewrite Heq1. erewrite typeOf_unbound. reflexivity.
-        apply H2. assumption. apply Heq1. assumption.
-      + destruct p. destruct (typeOf Rho e) eqn:Heq1; try discriminate.
-        destruct t; try discriminate.
-        destruct (eqType t0 t4 && eqType t3 t5) eqn:Heq2;
-        try discriminate. eapply anyIn_concat2 in H1.
-        destruct H1 as [H1 H2]. erewrite IHe.
-        rewrite Heq1. rewrite Heq2. shelve. apply Heq1.
-        apply H1. Unshelve.
-        apply andb_true_iff in Heq2. destruct Heq2 as [Heq2 Heq3].
-        apply eq_Type_eq in Heq2. apply eq_Type_eq in Heq3. subst.
-        destruct (Nat.eqb n1 n0) eqn:Heq3,
-                 (Nat.eqb n2 n1) eqn:Heq4.
-        * apply Nat.eqb_eq in Heq3. apply Nat.eqb_eq in Heq4. subst.
-          contradiction.
-        * apply Nat.eqb_eq in Heq3. apply Nat.eqb_neq in Heq4. subst.
-          rewrite double_update. reflexivity.
-        * apply Nat.eqb_neq in Heq3. apply Nat.eqb_eq in Heq4. subst.
-          rewrite double_update_indep. rewrite double_update.
-          rewrite double_update_indep. reflexivity.
-          assumption. symmetry. assumption.
-        * apply Nat.eqb_neq in Heq3. apply Nat.eqb_neq in Heq4.
-          erewrite (double_update_indep _ n1 _ n0).
-          erewrite (double_update_indep _ n1 _ n2).
-          erewrite typeOf_unbound. reflexivity.
-          apply H. apply anyIn_removeb in H2. apply anyIn_removeb in H2.
-          apply H2. assumption. symmetry. assumption.
-          symmetry. assumption. assumption.
+    - destruct (typeOf Rho e1) eqn:Heq1; try discriminate.
+      destruct t; try discriminate.
+      destruct (typeOf Rho e2) eqn:Heq2; try discriminate.
+      destruct (typeOf Rho e3) eqn:Heq3; try discriminate.
+      destruct (eqType t t0) eqn:Heq4; try discriminate.
+      apply eq_Type_eq in Heq4. subst.
+      inversion H. subst. eapply anyIn_concat2 in H1.
+      destruct H1 as [H3 H4].  apply anyIn_concat2 in H4.
+      destruct H4 as [H5 H6]. erewrite IHe1.
+      rewrite Heq1. erewrite IHe2. rewrite Heq2.
+      erewrite IHe3. rewrite Heq3. rewrite eqType_refl. reflexivity.
+      eassumption. eassumption. eassumption.
+      eassumption. eassumption. eassumption.
+    - destruct p, (typeOf Rho e1) eqn:Heq1; try discriminate.
+      simpl in H. destruct (eqType t (TList t0)) eqn:Heq2;
+      try discriminate. apply eq_Type_eq in Heq2. subst.
+      destruct (typeOf Rho e2) eqn:Heq3,
+               (typeOf (update Nat.eqb
+                  (update Nat.eqb Rho n2 (TList t0)) n0 t0)
+                  e3) eqn:Heq4; try discriminate.
+      simpl in H. destruct (eqType t t3) eqn:Heq5; try discriminate.
+      apply eq_Type_eq in Heq5. inversion H. subst.
+      eapply anyIn_concat2 in H1.
+      destruct H1 as [H1 H2]. apply anyIn_concat2 in H2.
+      destruct H2 as [H3 H4].
+      erewrite IHe1. shelve. eassumption. eassumption. Unshelve.
+      erewrite IHe2. shelve. eassumption. eassumption. Unshelve.
+      rewrite eqTypeS_refl. rewrite eqTypeS_refl.
+      rewrite Heq1. rewrite eqTypeS_refl.
+      rewrite Heq3.
+      destruct (Nat.eqb n1 n2) eqn:Heq6.
+      + rewrite Nat.eqb_eq in Heq6. subst n2.
+        rewrite double_update. rewrite Heq4.
+        rewrite eqTypeS_refl. reflexivity.
+      + destruct (Nat.eqb n1 n0) eqn:Heq7.
+        * apply Nat.eqb_neq in Heq6. apply Nat.eqb_eq in Heq7.
+          subst n0. rewrite (double_update_indep _ n1 _ n2).
+          rewrite double_update. rewrite Heq4.
+          rewrite eqTypeS_refl. reflexivity.
+          assumption.
+        * apply Nat.eqb_neq in Heq6. apply Nat.eqb_neq in Heq7.
+          rewrite (double_update_indep _ n1 _ n2).
+          rewrite (double_update_indep _ n1 _ n0).
+          erewrite IHe3. rewrite Heq4.
+          rewrite eqTypeS_refl. reflexivity.
+          eassumption. shelve. assumption.
+          assumption. Unshelve. apply anyIn_removeb in H4.
+          apply anyIn_removeb in H4. assumption.
+          symmetry. eassumption. symmetry. eassumption.
   Qed.
 
   Lemma any_in_subst :
@@ -1160,15 +1308,15 @@ Section PreservationTTypesHelper.
     anyIn (freeVars e2) (boundVars e3) = false ->
     anyIn (freeVars e2) (boundVars (subst n3 e3 e1)) = false.
   Proof.
-    fix any_in_subst 1.
-    --
     induction e1; intros e2 e3 n3 H1 H2 H3.
     - simpl. destruct (Nat.eqb n n3) eqn:Heq.
       * rewrite Nat.eqb_eq in Heq. subst n3.
         simpl in H1. apply H3.
       * apply H1.
     - simpl. apply H1.
-    - simpl. apply anyIn_Pair in H1. destruct H1.
+    - simpl. apply H1.
+    - simpl. apply H1.
+    - simpl. apply anyIn_Cons in H1. destruct H1.
       eapply anyIn_concat1_r. apply IHe1_1; assumption.
       apply IHe1_2; assumption.
     - simpl. apply anyIn_App in H1. destruct H1.
@@ -1183,26 +1331,34 @@ Section PreservationTTypesHelper.
     - simpl. apply anyIn_Or in H1. destruct H1.
       eapply anyIn_concat1_r. apply IHe1_1; assumption.
       apply IHe1_2; assumption.
-    - destruct b.
-      * simpl. apply anyIn_Case_Unit in H1. destruct H1.
-        eapply anyIn_concat1_r. apply IHe1; assumption.
-        apply any_in_subst; assumption.
-      * destruct p. simpl.
-        apply anyIn_Case_Pair in H1. destruct H1.
-        destruct (Nat.eqb n3 n1) eqn:Heq1,
-                 (Nat.eqb n3 n2) eqn:Heq2; simpl in *.
-        + apply Nat.eqb_eq in Heq1. apply Nat.eqb_eq in Heq2. subst.
-          eapply anyIn_concat1_r. apply IHe1; assumption. assumption.
-        + apply Nat.eqb_eq in Heq1. apply Nat.eqb_neq in Heq2. subst.
-          eapply anyIn_concat1_r. apply IHe1; assumption. assumption.
-        + apply Nat.eqb_neq in Heq1. apply Nat.eqb_eq in Heq2. subst.
-          eapply anyIn_concat1_r. apply IHe1; assumption. assumption.
-        + apply Nat.eqb_neq in Heq1. apply Nat.eqb_neq in Heq2.
-          eapply anyIn_concat1_r. apply IHe1; assumption.
-          apply anyIn_cons in H0. destruct H0.
-          apply anyIn_cons in H0. destruct H0.
-          apply anyIn_cons_r. apply anyIn_cons_r.
-          apply any_in_subst; assumption. assumption. assumption.
+    - simpl. apply anyIn_Case_Bool in H1. destruct H1.
+      destruct H0.
+      eapply anyIn_concat1_r. apply IHe1_1; assumption.
+      eapply anyIn_concat1_r. apply IHe1_2; assumption.
+      apply IHe1_3; assumption.
+    - destruct p. apply anyIn_Case_List in H1. destruct H1.
+      destruct H0. simpl.
+      destruct (Nat.eqb n3 n1) eqn:Heq1,
+                (Nat.eqb n3 n2) eqn:Heq2; simpl in *.
+      + apply Nat.eqb_eq in Heq1. apply Nat.eqb_eq in Heq2. subst.
+        eapply anyIn_concat1_r. apply IHe1_1; assumption.
+        eapply anyIn_concat1_r. apply IHe1_2; assumption.
+        assumption.
+      + apply Nat.eqb_eq in Heq1. apply Nat.eqb_neq in Heq2. subst.
+        eapply anyIn_concat1_r. apply IHe1_1; assumption.
+        eapply anyIn_concat1_r. apply IHe1_2; assumption.
+        assumption.
+      + apply Nat.eqb_neq in Heq1. apply Nat.eqb_eq in Heq2. subst.
+        eapply anyIn_concat1_r. apply IHe1_1; assumption.
+        eapply anyIn_concat1_r. apply IHe1_2; assumption.
+        assumption.
+      + apply Nat.eqb_neq in Heq1. apply Nat.eqb_neq in Heq2.
+        eapply anyIn_concat1_r. eapply IHe1_1; assumption.
+        eapply anyIn_concat1_r. eapply IHe1_2; assumption.
+        apply anyIn_cons in H1. destruct H1.
+        apply anyIn_cons in H1. destruct H1.
+        apply anyIn_cons_r. apply anyIn_cons_r.
+        eapply IHe1_3; try eassumption. assumption. assumption.
   Qed.
 
 End PreservationTTypesHelper.
@@ -1219,8 +1375,6 @@ Section PreservationTTypes.
     typeOf Rho e2 = Some t2 ->
     typeOf Rho (subst n e2 e1) = Some t.
   Proof.
-    fix subst_preservation 2.
-    --
     intros Rho e1. generalize dependent Rho.
     induction e1; intros Rho e2 n0 t1 t2 HF H H1.
     - unfold typeOf in H. inversion H. subst. clear H.
@@ -1231,16 +1385,23 @@ Section PreservationTTypes.
       + rewrite Nat.eqb_sym in Heq. simpl.
         rewrite Heq. reflexivity.
     - inversion H. simpl. reflexivity.
+    - inversion H. simpl. reflexivity.
+    - inversion H. simpl. reflexivity.
     - inversion H. simpl.
       remember (update Nat.eqb Rho n0 t2) as Rho'.
-      destruct (typeOf Rho' e1_1) eqn:Heq1,
-               (typeOf Rho' e1_2) eqn:Heq2; try discriminate.
-      subst Rho'. apply anyIn_cons in HF. destruct HF as [HF HFA].
-      apply anyIn_Pair in HF. destruct HF as [HF1 HF2].
-      erewrite IHe1_1. erewrite IHe1_2.
-      reflexivity. apply anyIn_cons_r; assumption. eassumption.
-      assumption. apply anyIn_cons_r; assumption. eassumption.
-      assumption.
+      destruct (typeOf Rho' e1_2) eqn:Heq2;
+      try discriminate; destruct t; try discriminate.
+      destruct (typeOf Rho' e1_1) eqn:Heq1;
+      try discriminate. simpl in H2.
+      destruct (eqType t0 t) eqn:Heq3; try discriminate.
+      apply eq_Type_eq in Heq3. inversion H2.
+      subst. apply anyIn_cons in HF.
+      destruct HF as [HF HFA].
+      apply anyIn_Cons in HF. destruct HF as [HF1 HF2].
+      erewrite IHe1_1 with (t := t).
+      erewrite (IHe1_2) with (t := TList t).
+      reflexivity. apply anyIn_cons_r; assumption.
+      eassumption. assumption. apply anyIn_cons_r; assumption. eassumption. assumption.
     - simpl. simpl in H.
       remember (update Nat.eqb Rho n0 t2) as Rho'.
       destruct (typeOf Rho' e1_1) eqn:Heq1,
@@ -1283,58 +1444,98 @@ Section PreservationTTypes.
       apply Heq2. apply H1. Unshelve.
       rewrite eqTypeS_refl. reflexivity.
     - simpl. simpl in H.
-      destruct b.
-      + remember (update Nat.eqb Rho n0 t2) as Rho'.
-        destruct (typeOf Rho' e1) eqn:Heq1; try discriminate.
-        destruct t; try discriminate.
-        apply anyIn_cons in HF. destruct HF as [HF HFA].
-        apply anyIn_Case_Unit in HF. destruct HF as [HF1 HF2].
-        erewrite IHe1. shelve. apply anyIn_cons_r; assumption.
-        subst. apply Heq1. eassumption. Unshelve. simpl.
-        eapply subst_preservation. apply anyIn_cons_r; assumption.
-        subst. apply H. apply H1.
-      + destruct p. remember (update Nat.eqb Rho n0 t2) as Rho'.
-        destruct (typeOf Rho' e1) eqn:Heq1; try discriminate.
-        destruct t; try discriminate.
-        destruct (eqType t0 t4 && eqType t3 t5) eqn:Heq2;
-        try discriminate. apply anyIn_cons in HF.
-        destruct HF as [HF HFA]. apply anyIn_Case_Pair in HF.
-        destruct HF as [HF1 HF2].
-        destruct (Nat.eqb n0 n1) eqn:HeqN1, (Nat.eqb n0 n2) eqn:HeqN2.
-        * apply Nat.eqb_eq in HeqN1. apply Nat.eqb_eq in HeqN2. subst.
-          simpl. erewrite IHe1. shelve.
-          apply anyIn_cons_r; assumption. apply Heq1.
-          eassumption. Unshelve. simpl.
-          rewrite Heq2. erewrite double_update.
-          erewrite double_update in H.
-          erewrite double_update in H.
-          assumption.
-        * apply Nat.eqb_eq in HeqN1. apply Nat.eqb_neq in HeqN2. subst.
-          simpl. erewrite IHe1. shelve.
-          apply anyIn_cons_r; assumption. apply Heq1.
-          eassumption. Unshelve. simpl.
-          rewrite Heq2. erewrite double_update in H. assumption.
-        * apply Nat.eqb_neq in HeqN1. apply Nat.eqb_eq in HeqN2. subst.
-          simpl. erewrite IHe1. shelve.
-          apply anyIn_cons_r; assumption. apply Heq1.
-          eassumption. Unshelve. simpl.
-          rewrite Heq2. erewrite double_update_indep in H.
-          rewrite double_update in H.
-          erewrite double_update_indep in H.
-          assumption. apply HeqN1. symmetry. apply HeqN1.
-        * apply Nat.eqb_neq in HeqN1. apply Nat.eqb_neq in HeqN2.
-          subst. simpl. erewrite IHe1. shelve.
-          apply anyIn_cons_r; assumption. apply Heq1.
-          eassumption. Unshelve. simpl.
-          apply anyIn_cons in HF2. destruct HF2.
-          apply anyIn_cons in H0. destruct H0.
-          rewrite Heq2. eapply subst_preservation.
-          apply anyIn_cons_r; assumption.
-          erewrite (double_update_indep _ n2 _ n0).
-          erewrite (double_update_indep _ n1 _ n0).
-          eassumption. symmetry. assumption. symmetry. assumption.
-          erewrite typeOf_unbound; try eassumption;
-          erewrite typeOf_unbound; eassumption.
+      remember (update Nat.eqb Rho n0 t2) as Rho'.
+      destruct (typeOf Rho' e1_1) eqn:Heq1;
+      try discriminate. destruct t; try discriminate.
+      destruct (typeOf Rho' e1_2) eqn:Heq2;
+      try discriminate.
+      destruct (typeOf Rho' e1_3) eqn:Heq3;
+      try discriminate.
+      destruct (eqType t t0) eqn:Heq4; try discriminate.
+      apply eq_Type_eq in Heq4. inversion H. subst.
+      apply anyIn_cons in HF. destruct HF as [HF HFA].
+      apply anyIn_Case_Bool in HF. destruct HF as [HF1 [HF2 HF3]].
+      erewrite IHe1_1. shelve. apply anyIn_cons_r; assumption. apply Heq1. eassumption. Unshelve.
+      erewrite IHe1_2. shelve. apply anyIn_cons_r; assumption. apply Heq2. eassumption. Unshelve.
+      erewrite IHe1_3. shelve. apply anyIn_cons_r; assumption. apply Heq3. eassumption. Unshelve.
+      rewrite eqType_refl. reflexivity.
+    - destruct p. simpl. simpl in H.
+      remember (update Nat.eqb Rho n0 t2) as Rho'.
+      assert (typeOf Rho' e1_1 = Some (TList t0)) as Heq1.
+      { destruct (typeOf Rho' e1_1) eqn:Heq1;
+        try discriminate; simpl in H.
+        destruct (eqType t (TList t0)) eqn:Heq2;
+        try discriminate. apply eq_Type_eq in Heq2.
+        subst. reflexivity.
+      }
+      rewrite Heq1 in H. rewrite eqTypeS_refl in H.
+      destruct (typeOf Rho' e1_2) eqn:Heq2,
+               (typeOf (update Nat.eqb
+                 (update Nat.eqb Rho' n2 (TList t0))
+                    n1 t0) e1_3) eqn:Heq3;
+      try discriminate. simpl in H.
+      destruct (eqType t t3) eqn:Heq4; try discriminate.
+      apply eq_Type_eq in Heq4. inversion H. subst.
+      apply anyIn_cons in HF.
+      destruct HF as [HF HFA].
+      apply anyIn_Case_List in HF.
+      destruct HF as [HF1 [HF2 HF3]].
+      destruct (Nat.eqb n0 n1) eqn:HeqN1,
+               (Nat.eqb n0 n2) eqn:HeqN2.
+      * apply Nat.eqb_eq in HeqN1.
+        apply Nat.eqb_eq in HeqN2. subst.
+        simpl. rewrite double_update in Heq3.
+        rewrite double_update in Heq3.
+        rewrite double_update.
+        rewrite Heq3. erewrite IHe1_1.
+        rewrite eqTypeS_refl.
+        erewrite IHe1_2. rewrite eqTypeS_refl. reflexivity.
+        apply anyIn_cons_r; assumption.
+        eassumption. eassumption.
+        apply anyIn_cons_r; assumption.
+        eassumption. eassumption.
+      * apply Nat.eqb_eq in HeqN1.
+        apply Nat.eqb_neq in HeqN2. subst. simpl.
+        rewrite double_update_indep in Heq3.
+        rewrite double_update in Heq3.
+        rewrite double_update_indep in Heq3.
+        erewrite Heq3. erewrite IHe1_1.
+        rewrite eqTypeS_refl.
+        erewrite IHe1_2. rewrite eqTypeS_refl. reflexivity.
+        apply anyIn_cons_r; assumption.
+        eassumption. eassumption.
+        apply anyIn_cons_r; assumption.
+        eassumption. eassumption. eassumption. symmetry. assumption.
+      * apply Nat.eqb_neq in HeqN1.
+        apply Nat.eqb_eq in HeqN2. subst. simpl.
+        rewrite double_update in Heq3.
+        erewrite Heq3. erewrite IHe1_1.
+        rewrite eqTypeS_refl.
+        erewrite IHe1_2. rewrite eqTypeS_refl. reflexivity.
+        apply anyIn_cons_r; assumption.
+        eassumption. eassumption.
+        apply anyIn_cons_r; assumption.
+        eassumption. eassumption.
+      * apply Nat.eqb_neq in HeqN1.
+        apply Nat.eqb_neq in HeqN2.
+        subst. simpl. erewrite IHe1_1. shelve.
+        apply anyIn_cons_r; assumption. apply Heq1.
+        eassumption. Unshelve. simpl.
+        rewrite (eqType_refl).
+        apply anyIn_cons in HF3. destruct HF3.
+        apply anyIn_cons in H0. destruct H0.
+        erewrite IHe1_2. shelve.
+        apply anyIn_cons_r; assumption. rewrite Heq2.
+        reflexivity. assumption. Unshelve.
+        erewrite IHe1_3. rewrite eqTypeS_refl.
+        reflexivity. apply anyIn_cons_r; assumption.
+        erewrite (double_update_indep _ n1 _ n0).
+        erewrite (double_update_indep _ n2 _ n0).
+        rewrite Heq3. reflexivity. symmetry. assumption.
+        symmetry. assumption.
+        erewrite typeOf_unbound; try eassumption.
+        erewrite typeOf_unbound; try eassumption.
+        erewrite typeOf_unbound; try eassumption.
   Qed.
 
   Lemma subst_preservation2 :
@@ -1370,43 +1571,45 @@ Section PreservationTTypes.
     typeOf Rho e = Some t ->
     typeOf Rho e' = Some t.
   Proof.
-    induction e using Exp_Branch_mut
-      with (P := fun e => forall e' Rho t,
-        step e = Some e' ->
-        typeOf Rho e = Some t ->
-        typeOf Rho e' = Some t)
-           (P0 := fun brs => forall e e' Rho t,
-        step (Case e brs) = Some e' ->
-        typeOf Rho (Case e brs) = Some t ->
-        typeOf Rho e' = Some t); intros; inversion H; subst.
+    induction e; intros; inversion H; subst.
     - destruct (step e1) eqn:Heq1, (step e2) eqn:Heq2;
       inversion H2; subst.
       + unfold typeOf. fold typeOf.
         unfold typeOf in H0. fold typeOf in H0.
-        destruct (typeOf Rho e1) eqn:Heq3,
-                 (typeOf Rho e2) eqn:Heq4;
-        try inversion H0; subst.
-        erewrite IHe1. apply H0. reflexivity. apply Heq3.
+        destruct (typeOf Rho e2) eqn:Heq3,
+                 (typeOf Rho e1) eqn:Heq4;
+        try inversion H0; subst;
+        destruct t0; try inversion H0.
+        destruct (eqType t1 t0) eqn:Heq5;
+        try discriminate. apply eq_Type_eq in Heq5. subst.
+        inversion H3. subst.
+        erewrite IHe1. apply H0. reflexivity. apply Heq4.
       + unfold typeOf. fold typeOf.
         unfold typeOf in H0. fold typeOf in H0.
-        destruct (typeOf Rho e1) eqn:Heq3,
-                 (typeOf Rho e2) eqn:Heq4;
-        try inversion H0; subst.
-        erewrite IHe1. apply H0. reflexivity. apply Heq3.
+        destruct (typeOf Rho e2) eqn:Heq3,
+                 (typeOf Rho e1) eqn:Heq4;
+        try inversion H0; subst;
+        destruct t0; try inversion H0.
+        destruct (eqType t1 t0) eqn:Heq5;
+        try discriminate. apply eq_Type_eq in Heq5. subst.
+        inversion H3. subst.
+        erewrite IHe1. apply H0. reflexivity. apply Heq4.
       + unfold typeOf. fold typeOf.
         unfold typeOf in H0. fold typeOf in H0.
-        destruct (typeOf Rho e1) eqn:Heq3,
-                 (typeOf Rho e2) eqn:Heq4;
-        try inversion H0; subst.
-        erewrite IHe2. apply H0. reflexivity. apply Heq4.
+        destruct (typeOf Rho e2) eqn:Heq3,
+                 (typeOf Rho e1) eqn:Heq4;
+        try inversion H0; subst;
+        destruct t0; try inversion H0.
+        destruct (eqType t1 t0) eqn:Heq5;
+        try discriminate. apply eq_Type_eq in Heq5. subst.
+        inversion H3. subst. erewrite IHe2 with (t := TList t0).
+        apply H0. reflexivity. apply Heq3.
   - destruct e1; try inversion H2.
-    + destruct (step (Pair e1_1 e1_2)) eqn:Heq1;
-      inversion H2; subst.
-      unfold typeOf. fold typeOf.
-      unfold typeOf in H0. fold typeOf in H0.
-      destruct (typeOf Rho e1_1) eqn:Heq2,
-               (typeOf Rho e1_2) eqn:Heq3;
-      try inversion H0; subst.
+    + simpl in H0.
+      destruct (typeOf Rho e1_2); try inversion H0.
+      destruct t0; try inversion H0.
+      destruct (eqTypeS (typeOf Rho e1_1) (Some t0));
+      try inversion H0.
     + destruct (step (App e1_1 e1_2)) eqn:Heq1;
       inversion H2; subst.
       unfold typeOf. fold typeOf.
@@ -1444,168 +1647,185 @@ Section PreservationTTypes.
       destruct (eqType t2_1 t0) eqn:Heq7; try inversion H0; subst.
       rewrite eq_Type_eq in Heq4. subst. rewrite Heq7.
       rewrite eqTypeS_refl. reflexivity.
-    + destruct e1; try inversion H3; subst.
-      * destruct b; try inversion H3; subst.
-        unfold typeOf. fold typeOf.
-        unfold typeOf in H0. fold typeOf in H0.
-        apply H0.
-      * destruct b; try inversion H3; subst.
-        destruct p. simpl in *. inversion H2.
-        unfold typeOf. fold typeOf.
-        destruct (typeOf Rho e1_1) eqn:Heq1,
-                 (typeOf Rho e1_2) eqn:Heq2; try inversion H0; subst.
-        destruct (eqType t1 t0 && eqType t2 t3) eqn:Heq3;
+    + destruct e1_1; try inversion H3; subst.
+      * simpl. simpl in H0.
+        destruct (typeOf Rho e1_2) eqn:Heq1,
+                 (typeOf Rho e1_3) eqn:Heq2; try inversion H0; subst.
+        destruct (eqType t0 t1) eqn:Heq3;
         try inversion H0; subst.
-        apply andb_true_iff in Heq3. destruct Heq3 as [Heq3_1 Heq3_2].
-        apply eq_Type_eq in Heq3_1. apply eq_Type_eq in Heq3_2. subst.
+        apply eq_Type_eq in Heq3. subst. reflexivity.
+      * simpl. simpl in H0.
+        destruct (typeOf Rho e1_2) eqn:Heq1,
+                 (typeOf Rho e1_3) eqn:Heq2; try inversion H0; subst.
+        destruct (eqType t0 t1) eqn:Heq3;
+        try inversion H0; subst.
+        apply eq_Type_eq in Heq3. subst. reflexivity.
+      * simpl. simpl in H0.
+        destruct (typeOf Rho e1_1_1) eqn:Heq1,
+                 (typeOf Rho e1_1_2) eqn:Heq2; try inversion H0.
+        simpl in H0. destruct (eqType t0 t1) eqn:Heq3;
+        try inversion H0; subst.
+        apply eq_Type_eq in Heq3. subst.
+        destruct t1; try inversion H0; subst.
+        destruct (typeOf Rho e1_2) eqn:Heq4; try inversion H0; subst.
+        destruct (typeOf Rho e1_3) eqn:Heq5; try inversion H0; subst.
+        destruct (eqType t0 t1) eqn:Heq6; try inversion H0; subst.
+        apply eq_Type_eq in Heq6. subst.
+        destruct t1; try inversion H0; subst.
+        destruct (typeOf Rho e2) eqn:Heq7; try inversion H0; subst.
+        destruct (eqType t1_1 t0) eqn:Heq8; try inversion H0; subst.
+        rewrite eq_Type_eq in Heq8. subst.
+        rewrite eqTypeS_refl. rewrite eqType_refl. reflexivity.
+    + destruct p, e1_1; inversion H3; subst.
+      * simpl. simpl in H0.
+        destruct (eqType t0 t1) eqn:Heq1;
+        try discriminate; subst.
+        destruct (typeOf Rho e1_2) eqn:Heq2; try discriminate;
         destruct (typeOf (update Nat.eqb
-                         (update Nat.eqb Rho n1 t0) n2 t3) e) eqn:Heq4;
-        try inversion H0; subst.
-        destruct t1; inversion H0; subst.
-        destruct (typeOf Rho e2) eqn:Heq5; try inversion H0; subst.
-        destruct (eqType t1_1 t1) eqn:Heq6; try inversion H0; subst.
-        destruct (anyIn (freeVars e1_1 ++ freeVars e1_2)
-                        (n1::n2:: boundVars e)) eqn:Heq7;
-        try inversion H2; subst.
-        destruct (anyIn (freeVars e1_2)(boundVars e1_1)) eqn:Heq8;
-        try inversion H2; subst. unfold typeOf. fold typeOf.
-        apply anyIn_concat2 in Heq7. destruct Heq7 as [Heq7_1 Heq7_2].
+                         (update Nat.eqb Rho n2 (TList t1))
+                         n1 t1) e1_3) eqn:Heq3;
+        try discriminate; subst. simpl in H0.
+        destruct (eqType t2 t3) eqn:Heq4; try discriminate; subst.
+        apply eq_Type_eq in Heq4. assumption.
+      * simpl. simpl in H0.
+        destruct (anyIn (freeVars e1_1_1 ++ freeVars e1_1_2)
+                        (n1 :: n2 :: boundVars e1_3)) eqn:Heq1;
+        try discriminate.
+        destruct (anyIn (freeVars e1_1_2)
+                        (boundVars e1_1_1)) eqn:Heq2;
+        try discriminate. inversion H3. subst.
+        apply anyIn_concat2 in Heq1. destruct Heq1 as [Heq1 HFA].
+        destruct (typeOf Rho e1_1_2) eqn:Heq3; try discriminate.
+        destruct t0; try discriminate; subst.
+        destruct (typeOf Rho e1_1_1) eqn:Heq4; try discriminate.
+        simpl in H0. simpl.
+        destruct (eqType t2 t0) eqn:Heq5; try discriminate.
+        apply eq_Type_eq in Heq5. subst. simpl. simpl in H0.
+        destruct (eqType t0 t1) eqn:Heq6; try discriminate.
+        apply eq_Type_eq in Heq6. subst.
+        destruct (typeOf Rho e1_2) eqn:Heq7; try discriminate;
+        destruct (typeOf (update Nat.eqb
+                         (update Nat.eqb Rho n2 (TList t1))
+                         n1 t1) e1_3) eqn:Heq8; try discriminate.
+        simpl in H0. destruct (eqType t0 t2) eqn:Heq9;
+        try discriminate. apply eq_Type_eq in Heq9. subst.
+        destruct t2; try discriminate; subst.
+        destruct (typeOf Rho e2) eqn:Heq10; try discriminate.
+        destruct (eqType t2_1 t0) eqn:Heq11; try discriminate.
+        apply eq_Type_eq in Heq11. subst. inversion H0. subst.
+        simpl in H2.
         erewrite subst_preservation2. shelve.
-        assumption. assumption. assumption. symmetry. assumption.
-        apply Heq4. apply  Heq2. apply Heq1. Unshelve.
-        simpl. rewrite Heq5. rewrite Heq6. reflexivity.
-      * unfold typeOf. fold typeOf.
-        unfold typeOf in H0. fold typeOf in H0.
-        destruct b.
-        --  destruct (eqTypeS (typeOf Rho e1_1)
-                              (typeOf Rho e1_2)) eqn:Heq1;
-            try inversion H0; subst.
-            destruct (typeOf Rho e1_1) eqn:Heq2;
-            destruct (typeOf Rho e1_2) eqn:Heq3;
-            try inversion H0; try inversion Heq1.
-            destruct t0; inversion H0; subst.
-            destruct t1; inversion Heq1; subst.
-            rewrite eqTypeS_refl. reflexivity.
-        --  destruct p.
-            destruct (eqTypeS (typeOf Rho e1_1) (typeOf Rho e1_2)) eqn:Heq1;
-            try inversion H0; subst.
-            destruct (typeOf Rho e1_1) eqn:Heq2;
-            destruct (typeOf Rho e1_2) eqn:Heq3;
-            try inversion H0; try inversion Heq1.
-            apply eq_Type_eq in Heq1. subst.
-            destruct t3; inversion H0; subst.
-            destruct (eqType t1 t3_1 && eqType t2 t3_2) eqn:Heq4;
-            try inversion H0; subst.
-            apply andb_true_iff in Heq4.
-            destruct Heq4 as [Heq4_1 Heq4_2].
-            apply eq_Type_eq in Heq4_1. apply eq_Type_eq in Heq4_2.
-            rewrite eqTypeS_refl. reflexivity.
-  - destruct (step e1) eqn:Heq1, (step e2) eqn:Heq2;
-    inversion H2; subst.
-    + unfold typeOf. fold typeOf.
-      unfold typeOf in H0. fold typeOf in H0.
-      destruct (typeOf Rho e1) eqn:Heq3,
-               (typeOf Rho e2) eqn:Heq4;
+        assumption. assumption. assumption.
+        symmetry. assumption.
+        rewrite double_update_indep. eassumption.
+        assumption. assumption. assumption.
+        Unshelve. simpl. rewrite eqType_refl. reflexivity.
+      * simpl. simpl in H0.
+        destruct (typeOf Rho e1_1_1) eqn:Heq4; try discriminate;
+        destruct (typeOf Rho e1_1_2) eqn:Heq3; try discriminate.
+        simpl in H0.
+        destruct (eqType t0 t2) eqn:Heq5; try discriminate.
+        apply eq_Type_eq in Heq5. subst. simpl. simpl in H0.
+        destruct (eqType t2 (TList t1)) eqn:Heq6; try discriminate.
+        apply eq_Type_eq in Heq6. subst.
+        destruct (typeOf Rho e1_2) eqn:Heq7; try discriminate;
+        destruct (typeOf (update Nat.eqb
+                         (update Nat.eqb Rho n2 (TList t1))
+                         n1 t1) e1_3) eqn:Heq8; try discriminate.
+        simpl in H0. destruct (eqType t0 t2) eqn:Heq9;
+        try discriminate. apply eq_Type_eq in Heq9. subst.
+        destruct t2; try discriminate; subst.
+        destruct (typeOf Rho e2) eqn:Heq10; try discriminate.
+        destruct (eqType t2_1 t0) eqn:Heq11; try discriminate.
+        apply eq_Type_eq in Heq11. subst. inversion H0. subst.
+        rewrite eqTypeS_refl. rewrite eqTypeS_refl.
+        rewrite eqType_refl. reflexivity.
+  - unfold typeOf in H0. fold typeOf in H0.
+    destruct (typeOf Rho e1) eqn:Heq1;
+    destruct (typeOf Rho e2) eqn:Heq2; try inversion H0; subst.
+    simpl in *.
+    destruct (eqType t0 t1) eqn:Heq3; try inversion H0; subst.
+    apply eq_Type_eq in Heq3. subst.
+    destruct (step e1) eqn:HeqS1.
+    + inversion H2. subst. simpl.
+      erewrite IHe1. erewrite Heq2. rewrite eqTypeS_refl.
+      reflexivity. reflexivity. assumption.
+    + destruct (step e2) eqn:HeqS2.
+      * inversion H2. subst. simpl.
+        erewrite (IHe2 e). erewrite Heq1. rewrite eqTypeS_refl.
+        reflexivity. reflexivity. assumption.
+      * inversion H2.
+  - destruct e1; inversion H2; subst.
+    + simpl in H0. destruct (typeOf Rho e2) eqn:Heq1;
       try inversion H0; subst.
-      destruct (eqType t0 t1) eqn:Heq5; try inversion H3; subst.
-      apply eq_Type_eq in Heq5. subst.
-      erewrite IHe1. shelve. reflexivity. apply Heq3.
-      Unshelve. rewrite eqTypeS_refl. reflexivity.
-    + unfold typeOf. fold typeOf.
-      unfold typeOf in H0. fold typeOf in H0.
-      destruct (typeOf Rho e1) eqn:Heq3,
-               (typeOf Rho e2) eqn:Heq4;
-      try inversion H0; subst.
-      destruct (eqType t0 t1) eqn:Heq5; try inversion H3; subst.
-      apply eq_Type_eq in Heq5. subst.
-      erewrite IHe1. shelve. reflexivity. apply Heq3.
-      Unshelve. rewrite eqTypeS_refl. reflexivity.
-    + unfold typeOf. fold typeOf.
-      unfold typeOf in H0. fold typeOf in H0.
-      destruct (typeOf Rho e1) eqn:Heq3,
-               (typeOf Rho e2) eqn:Heq4;
-      try inversion H0; subst.
-      destruct (eqType t0 t1) eqn:Heq5; try inversion H3; subst.
-      apply eq_Type_eq in Heq5. subst.
-      erewrite IHe2. shelve. reflexivity. apply Heq4.
-      Unshelve. rewrite eqTypeS_refl. reflexivity.
-  - destruct e; inversion H2; subst.
-    + destruct b; inversion H3; subst.
-      unfold typeOf. fold typeOf.
-      unfold typeOf in H0. fold typeOf in H0.
-      assumption.
-    + destruct b; inversion H3; subst. destruct p.
-      unfold typeOf. fold typeOf.
-      unfold typeOf in H0. fold typeOf in H0.
-      destruct (typeOf Rho e1) eqn:Heq1;
-      destruct (typeOf Rho e2) eqn:Heq2; try inversion H0; subst.
-      destruct (eqType t1 t0 && eqType t2 t3) eqn:Heq3;
-      try inversion H0; subst.
-      erewrite IHe0. rewrite H5. reflexivity.
-      apply H. unfold typeOf. fold typeOf.
-      rewrite Heq1. rewrite Heq2. rewrite Heq3.
-      apply H5.
-    + unfold typeOf. fold typeOf.
-      unfold typeOf in H0. fold typeOf in H0.
-      destruct b.
-      * destruct (eqTypeS (typeOf Rho e1) (typeOf Rho e2)) eqn:Heq1;
-        try inversion H0; subst.
-        destruct (typeOf Rho e1) eqn:Heq2;
-        destruct (typeOf Rho e2) eqn:Heq3;
-        try inversion H0; try inversion Heq1.
-        destruct t0; inversion H0; subst.
-        destruct t1; inversion Heq1; subst.
-        rewrite eqTypeS_refl. reflexivity.
-      * destruct p.
-        destruct (eqTypeS (typeOf Rho e1) (typeOf Rho e2)) eqn:Heq1;
-        try inversion H0; subst.
-        destruct (typeOf Rho e1) eqn:Heq2;
-        destruct (typeOf Rho e2) eqn:Heq3;
-        try inversion H0; try inversion Heq1.
-        destruct t0; inversion H0; subst.
-        destruct (eqType t1 t0_1 && eqType t2 t0_2) eqn:Heq4;
-        try inversion H0; subst. rewrite H6.
-        apply eq_Type_eq in H5. subst. rewrite Heq4.
-        rewrite eqTypeS_refl. reflexivity.
-  - destruct e0; inversion H2.
-    + unfold typeOf in H0. fold typeOf in H0.
-      subst. assumption.
-    + unfold typeOf in H0. fold typeOf in H0.
-      unfold typeOf. fold typeOf.
-      destruct (typeOf Rho e0_1) eqn:Heq1;
-      destruct (typeOf Rho e0_2) eqn:Heq2; try inversion H0; subst.
-      simpl in *.
+      destruct (typeOf Rho e') eqn:Heq2; try inversion H0; subst.
       destruct (eqType t0 t1) eqn:Heq3; try inversion H0; subst.
+      apply eq_Type_eq in Heq3. subst. reflexivity.
+    + simpl in H0. destruct (typeOf Rho e') eqn:Heq1,
+             (typeOf Rho e3) eqn:Heq2; try inversion H0; subst.
+      destruct (eqType t0 t1) eqn:Heq3; try inversion H0; subst.
+      apply eq_Type_eq in Heq3. subst. reflexivity.
+    + simpl. simpl in H0. destruct (typeOf Rho e1_1) eqn:Heq1;
+      destruct (typeOf Rho e1_2) eqn:Heq2; try inversion H0; subst.
+      simpl in H0. destruct (eqType t0 t1) eqn:Heq3;
+      try inversion H0; subst. destruct t0; try inversion H0; subst.
       apply eq_Type_eq in Heq3. subst.
-      destruct t1; inversion H0; subst.
+      destruct (typeOf Rho e2) eqn:Heq4; try inversion H0; subst.
+      destruct (typeOf Rho e3) eqn:Heq5; try inversion H0; subst.
+      destruct (eqType t0 t1) eqn:Heq6; try inversion H0; subst.
+      apply eq_Type_eq in Heq6. subst.
       rewrite eqTypeS_refl. reflexivity.
-  - destruct p. destruct e0; inversion H2; subst.
-    + unfold typeOf in H0. fold typeOf in H0.
-      unfold typeOf. fold typeOf.
-      destruct (typeOf Rho e0_1) eqn:Heq1;
-      destruct (typeOf Rho e0_2) eqn:Heq2; try inversion H0; subst.
-      simpl in *.
-      destruct (eqType t1 t0 && eqType t2 t3) eqn:Heq3; try inversion H0; subst.
-      apply andb_true_iff in Heq3. destruct Heq3 as [Heq4 Heq5].
-      apply eq_Type_eq in Heq4. apply eq_Type_eq in Heq5. subst.
-      destruct (anyIn (freeVars e0_1 ++ freeVars e0_2)
-                      (n1::n2::boundVars e)) eqn:Heq6;
-      try inversion H2; subst.
-      destruct (anyIn (freeVars e0_2) (boundVars e0_1)) eqn:Heq7;
-      try inversion H2; subst.
-      apply anyIn_concat2 in Heq6. destruct Heq6 as [Heq6_1 Heq6_2].
-      erewrite subst_preservation2. rewrite H0. reflexivity.
-      assumption. assumption. assumption. symmetry. assumption.
-      apply H0. apply Heq2. apply Heq1.
-    + unfold typeOf in H0. fold typeOf in H0.
-      unfold typeOf. fold typeOf.
-      destruct (typeOf Rho e0_1) eqn:Heq1;
-      destruct (typeOf Rho e0_2) eqn:Heq2; try inversion H0; subst.
-      simpl in *.
-      destruct (eqType t0 t3) eqn:Heq3; try inversion H0; subst.
-      apply eq_Type_eq in Heq3. subst.
-      destruct t3; inversion H0; subst.
+  - destruct p. destruct e1; inversion H2; subst.
+    + simpl in H0. destruct (eqType t0 t1) eqn:Heq1;
+      try inversion H0; subst.
+      apply eq_Type_eq in Heq1. subst.
+      destruct (typeOf Rho e') eqn:Heq2; try inversion H0; subst;
+      destruct (typeOf (update Nat.eqb
+                       (update Nat.eqb Rho n2 (TList t1))
+                       n1 t1) e3) eqn:Heq3; try inversion H0; subst.
+      destruct (eqType t0 t2) eqn:Heq4; try inversion H4; subst.
+      apply eq_Type_eq in Heq4. subst.
       rewrite eqTypeS_refl. reflexivity.
+    + destruct (anyIn (freeVars e1_1 ++ freeVars e1_2)
+                      (n1 :: n2 :: boundVars e3)) eqn:Heq1;
+      try inversion H2; subst.
+      destruct (anyIn (freeVars e1_2) (boundVars e1_1)) eqn:Heq2;
+      try inversion H2; subst.
+      apply anyIn_concat2 in Heq1. destruct Heq1 as [Heq1 HFA].
+      simpl in H0.
+      destruct (typeOf Rho e1_2) eqn:Heq3; try inversion H0; subst.
+      destruct t0; try inversion H0; subst.
+      destruct (typeOf Rho e1_1) eqn:Heq4; try inversion H0; subst.
+      simpl in H0. simpl.
+      destruct (eqType t2 t0) eqn:Heq5; try inversion H0; subst.
+      apply eq_Type_eq in Heq5. subst.
+      destruct (eqType t0 t1) eqn:Heq6; try inversion H8; subst.
+      apply eq_Type_eq in Heq6. subst.
+      destruct (typeOf Rho e2) eqn:Heq7; try inversion H8; subst;
+      destruct (typeOf (update Nat.eqb
+                       (update Nat.eqb Rho n2 (TList t1))
+                       n1 t1) e3) eqn:Heq8; try inversion H10; subst.
+      destruct (eqType t0 t2) eqn:Heq9; try inversion H10; subst.
+      apply eq_Type_eq in Heq9. subst.
+      rewrite eqTypeS_refl. rewrite eqTypeS_refl.
+      eapply subst_preservation2; try assumption.
+      symmetry. assumption.
+      rewrite double_update_indep. eassumption.
+      assumption. assumption. assumption.
+    + simpl. simpl in H0. destruct (typeOf Rho e1_1) eqn:Heq1;
+      destruct (typeOf Rho e1_2) eqn:Heq2; try inversion H0; subst.
+      simpl in H0. destruct (eqType t0 t2) eqn:Heq3;
+      try inversion H0; subst.
+      apply eq_Type_eq in Heq3. subst. simpl in H0.
+      destruct (eqType t2 (TList t1)) eqn:Heq4;
+      try inversion H0; subst. rewrite eq_Type_eq in Heq4. subst.
+      destruct (typeOf Rho e2) eqn:Heq4; try inversion H0; subst;
+      destruct (typeOf (update Nat.eqb
+                       (update Nat.eqb Rho n2 (TList t1))
+                       n1 t1) e3) eqn:Heq8; try inversion H0; subst.
+      destruct (eqType t0 t2) eqn:Heq6; try inversion H6; subst.
+      apply eq_Type_eq in Heq6. subst.
+      rewrite eqTypeS_refl. rewrite eqTypeS_refl. reflexivity.
   Qed.
 
   Lemma well_typed_step :
@@ -1639,260 +1859,239 @@ End PreservationTTypes.
 Section Proofs.
 
   Lemma compatibility:
-    forall e Rho Gamma x,
-    Gamma = mkCompatibleCtx Rho ->
-    well_typed Rho e ->
-    Gamma |- e ::: x ->
-    exists t,
-    typeOf Rho e = Some t /\
-    compatible x t.
+    forall e Rho Gamma t d,
+    compatibleCtx Gamma Rho ->
+    typeOf Rho e = Some t ->
+    Gamma |- e ::: d ->
+    compatible d t.
   Proof.
-    induction e using Exp_Branch_mut
-      with (P :=  fun e => forall Rho Gamma x,
-                    Gamma = mkCompatibleCtx Rho ->
-                    well_typed Rho e ->
-                    Gamma |- e ::: x -> exists t,
-                    typeOf Rho e = Some t /\
-                    compatible x t)
-           (P0 := fun brs => forall e Rho Gamma x,
-                    Gamma = mkCompatibleCtx Rho ->
-                    well_typed Rho (Case e brs) ->
-                    Gamma |- Case e brs ::: x -> exists t,
-                    typeOf Rho (Case e brs) = Some t /\
-                    compatible x t); intros.
+    induction e; intros.
     - inversion H1; subst.
-      unfold typeOf. fold typeOf.
-      unfold mkCompatibleCtx in *.
-      destruct (Rho n).
-        * eexists. split. reflexivity. reflexivity.
-        * eexists. split. reflexivity. apply mkCompatible_compatible.
-        * eexists. split. reflexivity. apply mkCompatible_compatible.
-    - inversion H1; subst. simpl in H1. exists TUnit.
-      split. reflexivity. reflexivity.
+      unfold typeOf in H0. inversion H0.
+      unfold compatibleCtx in *.
+      destruct (Rho n) eqn:HeqR; rewrite <- HeqR; apply H.
+    - inversion H1; subst. simpl in H1. simpl in H0. inversion H0.
+      reflexivity.
+    - inversion H1; subst. simpl in H1. simpl in H0. inversion H0.
+      reflexivity.
+    - inversion H1; subst. simpl in H1. simpl in H0. inversion H0.
+      reflexivity.
     - inversion H1. subst. simpl.
-      apply well_typed_Pair in H0.
-      destruct H0.
-      unfold well_typed in H0.
-      unfold well_typed in H.
-      destruct (typeOf Rho e1) eqn:Heq1;
-      destruct (typeOf Rho e2) eqn:Heq2;
-      try inversion H0; try inversion H.
-      exists (TPair t t0).
-      split. reflexivity. destruct d1; destruct d2; auto.
-    - remember H0 as H0C. clear HeqH0C.
-      unfold well_typed in H0.
-      unfold typeOf in *. fold typeOf in *.
-      destruct (typeOf Rho e1) eqn:Heq1.
-      shelve. inversion H0. Unshelve.
-      destruct t. inversion H0. inversion H0.
-      destruct (typeOf Rho e2).
-      shelve. inversion H0. Unshelve.
-      destruct (eqType t1 t).
-      shelve. inversion H0. Unshelve.
-      exists t2. inversion H1; subst.
-      + split. reflexivity. reflexivity.
-      + unfold decide in H1. unfold decide.
-        destruct (more_specific d3 d1) eqn:Heq2.
-        * split. reflexivity.
-          apply well_typed_App in H0C. destruct H0C.
-          edestruct IHe1. reflexivity. apply H.
-          apply H4. destruct H3. rewrite Heq1 in H3.
-          inversion H3. subst. simpl in H5.
-          destruct H5. assumption.
-        * split. reflexivity. reflexivity.
+      simpl in H0.
+      destruct (typeOf Rho e2) eqn:Heq1;
+      destruct (typeOf Rho e1) eqn:Heq2;
+      try inversion H0; try inversion H2; subst;
+      destruct t0; try inversion H3.
+      destruct (eqType t1 t0) eqn:Heq3;
+      try inversion H3. apply eq_Type_eq in Heq3. subst.
+      inversion H3. destruct d1; destruct d2; auto; reflexivity.
+    - inversion H1; subst.
+      + reflexivity.
+      + unfold typeOf in *. fold typeOf in *.
+        destruct (typeOf Rho e1) eqn:Heq1.
+        shelve. inversion H0. Unshelve.
+        destruct t0. inversion H0. inversion H0.
+        destruct (typeOf Rho e2) eqn:Heq2.
+        shelve. inversion H0. Unshelve.
+        destruct (eqType t0_1 t0) eqn:Heq3.
+        shelve. inversion H0. Unshelve.
+        apply eq_Type_eq in Heq3. subst.
+        inversion H0; subst.
+        unfold decide in H1. unfold decide.
+        destruct (more_specific d3 d1) eqn:Heq3.
+        * eapply IHe1 in H4. shelve. eassumption. apply Heq1.
+          Unshelve. simpl in H4. destruct H4. assumption.
+        * reflexivity.
     - inversion H1. subst.
       remember H0 as H0C. clear HeqH0C.
       unfold well_typed in H0.
       destruct (typeOf Rho (Abs n t e)) eqn:Heq1.
       + unfold typeOf in Heq1. fold typeOf in Heq1.
         destruct (typeOf (update Nat.eqb Rho n t) e) eqn:Heq2.
-        * exists t0. split. reflexivity. simpl.
-          inversion Heq1. subst.
-          apply well_typed_Abs in H0C.
-          edestruct IHe. reflexivity.
-          apply H0C. inversion H1.
-          subst Gamma'0. subst. erewrite <- update_compatible.
-          apply H9. reflexivity.
-          destruct H. rewrite Heq2 in H. inversion H. subst.
-          split. apply mkCompatible_compatible. assumption.
+        * simpl. inversion Heq1. inversion H0C. subst.
+          split. assumption.
+          eapply IHe. shelve. apply Heq2.
+          apply H8. Unshelve. subst Gamma'.
+          apply update_compatible. assumption.
+          assumption.
         * inversion Heq1.
       + inversion H0.
-    - inversion H1. unfold well_typed in H0.
-      destruct (typeOf Rho (Or e1 e2)). exists t.
-      split. reflexivity. reflexivity. inversion H0.
     - inversion H1.
-      + unfold well_typed in H0.
-        destruct b; inversion H3. subst.
-        destruct (typeOf Rho (Case e (BranchUnit e0))).
-        exists t. split; reflexivity. inversion H0.
-      + unfold well_typed in H0.
-        destruct b; inversion H4. subst.
-        destruct (typeOf Rho (Case e (BranchPair p e0))).
-        exists t. split; reflexivity.
-        inversion H0.
-      + subst. remember H0 as H0C. clear HeqH0C.
-        apply well_typed_Case_Unit in H0.
-        destruct H0 as [H0A H0B].
-        edestruct (IHe0 e Rho (mkCompatibleCtx Rho) x).
-        reflexivity. assumption. assumption.
-        destruct H. unfold well_typed in *.
-        unfold typeOf. fold typeOf.
-        unfold typeOf in H0C. fold typeOf in H0C.
-        destruct (typeOf Rho e) eqn:Heq1;
-        destruct (typeOf Rho e2) eqn:Heq2;
-        try inversion H0A; try inversion H0B.
-        destruct t; try inversion H0C.
-        inversion H. subst.
-        exists x0. split. rewrite Heq2 in H3. rewrite Heq1 in H3.
-        assumption. assumption.
-      + subst. remember H0 as H0C. clear HeqH0C.
-        remember H0 as H0D. clear HeqH0D.
-        unfold well_typed in H0.
-        unfold typeOf in H0. fold typeOf in H0.
-        unfold typeOf. fold typeOf.
-        destruct (typeOf Rho e) eqn:Heq1.
-        shelve. inversion H0. Unshelve. subst.
-        destruct p. destruct t; try inversion H0.
-        remember (update Nat.eqb Rho n0 t0) as Rho'.
-        destruct (eqType t0 t4 && eqType t3 t5) eqn:Heq3.
-        shelve. inversion H0. Unshelve.
-        destruct (typeOf (update Nat.eqb Rho' n3 t3) e2) eqn:Heq2.
-        shelve. inversion H0. Unshelve.
-        eapply well_typed_Case_Pair in H0C.
-        destruct H0C.
-        edestruct (IHe0 e). reflexivity. apply H0D.
-        apply H1. destruct H4. exists t. split. reflexivity.
-        unfold typeOf in H4. fold typeOf in H4.
-        rewrite Heq1 in H4. rewrite Heq3 in H4.
-        subst Rho'. rewrite Heq2 in H4.
-        inversion H4. subst. assumption.
+      destruct (typeOf Rho (Or e1 e2)); reflexivity.
     - inversion H1; subst.
-      + unfold well_typed in H0.
-        destruct (typeOf Rho (Case e0 (BranchUnit e))) eqn:Heq1.
-        exists t. split; reflexivity.
-        inversion H0.
-      + remember H0 as H0C. clear HeqH0C.
-        unfold well_typed in H0.
-        apply well_typed_Case_Unit in H0C.
-        destruct H0C as [H0A H0B].
-        destruct (typeOf Rho (Case e0 (BranchUnit e))) eqn:Heq1.
-        shelve. inversion H0. Unshelve.
-        exists t. edestruct (IHe Rho). reflexivity.
-        apply H0B. apply H7. destruct H.
-        unfold typeOf in Heq1. fold typeOf in Heq1.
-        rewrite H in Heq1. destruct (typeOf Rho e0) eqn:Heq2.
-        shelve. inversion Heq1. Unshelve.
-        destruct t0; inversion Heq1. subst.
-        split. reflexivity. assumption.
+      simpl in H0.
+      destruct (typeOf Rho e1) eqn:Heq1;
+      try discriminate; destruct t0;
+      destruct (typeOf Rho e2) eqn:Heq2;
+      destruct (typeOf Rho e3) eqn:Heq3;
+      try discriminate.
+      destruct (eqType t0 t1) eqn:Heq4;
+      try discriminate; apply eq_Type_eq in Heq4; subst.
+      eapply (IHe1 _ _ _ _ H Heq1) in H6.
+      eapply (IHe2 _ _ _ _ H Heq2) in H8.
+      eapply (IHe3 _ _ _ _ H Heq3) in H9.
+      inversion H0. subst.
+      apply compatible_lub; assumption.
     - inversion H1; subst.
-      + unfold well_typed in H0.
-        destruct (typeOf Rho (Case e0 (BranchPair p0 e))) eqn:Heq1.
-        exists t. split; reflexivity. inversion H0.
-      + subst p0. remember H0 as H0C. clear HeqH0C.
-        unfold well_typed in H0.
-        apply well_typed_Case_Pair in H0C.
-        destruct H0C as [H0A H0B].
-        remember (BranchPair (Pat n1 t1 n2 t2 H2) e) as b.
-        destruct (typeOf Rho (Case e0 b)) eqn:Heq1.
-        shelve. inversion H0. Unshelve.
-        exists t. edestruct (IHe). reflexivity.
-        apply H0B. subst Gamma''. subst Gamma'.
-        erewrite <- update_update_compatible.
-        apply H9. reflexivity. destruct H. subst b.
-        unfold typeOf in Heq1. fold typeOf in Heq1.
-        rewrite H in Heq1. destruct (typeOf Rho e0) eqn:Heq2.
-        shelve. inversion Heq1. Unshelve.
-        destruct t0; inversion Heq1.
-        destruct (eqType t1 t0_1 && eqType t2 t0_2) eqn:Heq3.
-        shelve. inversion Heq1. Unshelve.
-        split. reflexivity. inversion H5. subst. assumption.
+      simpl in H0.
+      destruct (typeOf Rho e1) eqn:Heq1;
+      try discriminate. simpl in H0.
+      destruct (eqType t0 (TList t1)) eqn:Heq2;
+      try discriminate; apply eq_Type_eq in Heq2; subst.
+      destruct (typeOf Rho e2) eqn:Heq3;
+      try discriminate;
+      destruct (typeOf (update Nat.eqb
+                  (update Nat.eqb Rho n2 (TList t1))
+                  n1 t1) e3) eqn:Heq4;
+      try discriminate; subst. simpl in H0.
+      destruct (eqType t0 t2) eqn:Heq5;
+      try discriminate; apply eq_Type_eq in Heq5; subst.
+      inversion H0; subst.
+      eapply (IHe1 _ _ _ _ H Heq1) in H7.
+      eapply (IHe2 _ _ _ _ H Heq3) in H12.
+      eapply (IHe3) in H13.
+      apply compatible_lub; try assumption.
+      destruct d_1; try assumption.
+      apply H13. shelve.
+      apply Heq4. Unshelve. subst Gamma'. subst Gamma''.
+      destruct (Nat.eqb n1 n2) eqn:HeqN1.
+      + apply Nat.eqb_eq in HeqN1. subst.
+        contradiction.
+      + apply Nat.eqb_neq in HeqN1.
+        rewrite double_update_indep.
+        apply update_compatible.
+        apply update_compatible.
+        apply H. apply H11. apply H9.
+        apply HeqN1.
   Qed.
+
 
   (* Theorem completeness:
     Shows that any well-typed expression in the Curry type system
     can be assigned a determinism type. This establishes that
     determinism typing covers all valid programs. *)
   Theorem completeness :
-    forall e Rho Gamma,
-    Gamma = mkCompatibleCtx Rho ->
-    well_typed Rho e ->
-    exists d, Gamma |- e ::: d.
+    forall e Rho Gamma t,
+    compatibleCtx Gamma Rho ->
+    typeOf Rho e = Some t ->
+    exists d, Gamma |- e ::: d /\ compatible d t.
   Proof.
-    fix completeness 1.
     intro e.
-    induction e; intros Rho Gamma HG HW.
+    induction e; intros Rho Gamma t0 HG HW.
     * destruct (Gamma n) eqn:Heq.
-        - exists D. apply Rule_Var.
+        - exists D. split. apply Rule_Var.
           rewrite Heq. reflexivity.
-        - exists ND. apply Rule_Var.
+          eapply compatibility in HW. apply HW.
+          eassumption. eapply Rule_Var. assumption.
+        - exists ND. split. apply Rule_Var.
+          rewrite Heq. reflexivity. reflexivity.
+        - exists (Arrow d1 d2). split. apply Rule_Var.
           rewrite Heq. reflexivity.
-        - exists (Arrow d1 d2). apply Rule_Var.
-          rewrite Heq. reflexivity.
-    * exists D. apply Rule_Unit. reflexivity.
-    * apply well_typed_Pair in HW. destruct HW as [HW1 HW2].
-      destruct (IHe1 Rho Gamma HG HW1).
-      destruct (IHe2 Rho Gamma HG HW2).
-      destruct x; destruct x0; eexists; eapply Rule_Pair;
-      try eassumption; try reflexivity.
+          eapply compatibility in HW. apply HW.
+          eassumption. eapply Rule_Var. assumption.
+    * exists D. split. apply Rule_BTrue.
+      simpl in HW. inversion HW. reflexivity.
+    * exists D. split. apply Rule_BFalse.
+      simpl in HW. inversion HW. reflexivity.
+    * exists D. split. apply Rule_Nil.
+      simpl in HW. inversion HW. reflexivity.
+    * unfold typeOf in HW. fold typeOf in HW.
+      destruct (typeOf Rho e2) eqn:Heq1,
+               (typeOf Rho e1) eqn:Heq2; try inversion HW; subst;
+      destruct t; try inversion HW.
+      destruct (eqType t1 t) eqn:Heq3; try inversion H1.
+      apply eq_Type_eq in Heq3. subst.
+      destruct (IHe1 Rho Gamma t HG Heq2). destruct H.
+      destruct (IHe2 Rho Gamma _ HG Heq1). destruct H3.
+      eexists. split.
+      eapply Rule_Cons; try eassumption; try reflexivity.
+      destruct x; destruct x0; reflexivity.
     * remember HW as HWC. clear HeqHWC.
-      apply well_typed_App in HW. destruct HW as [HW1 HW2].
-      destruct (IHe1 Rho Gamma HG HW1).
-      destruct (IHe2 Rho Gamma HG HW2).
+      unfold typeOf in HWC. fold typeOf in HWC.
+      destruct (typeOf Rho e1) eqn:Heq1;
+      destruct (typeOf Rho e2) eqn:Heq2;
+      try inversion HWC; destruct t; try inversion HWC; subst.
+      destruct (eqType t2 t1) eqn:Heq3; try inversion HWC; subst.
+      apply eq_Type_eq in Heq3. subst.
+      destruct (IHe1 Rho Gamma (TArrow t1 t0) HG Heq1). destruct H.
+      destruct (IHe2 Rho Gamma t1 HG Heq2). destruct H3.
       destruct x.
-      - edestruct compatibility. eassumption. apply HW1.
-        apply H. destruct H1.
-        unfold well_typed in HWC.
-        unfold typeOf in HWC. fold typeOf in HWC.
-        rewrite H1 in HWC. destruct x; inversion H2; inversion HWC.
-      - exists ND. eapply Rule_AppND. apply H. apply H0.
-      - eexists. eapply Rule_AppND. apply H. apply H0.
-    * apply well_typed_Abs in HW.
-      edestruct (IHe (update Nat.eqb Rho n t) (update Nat.eqb Gamma n (mkCompatible t))). shelve. apply HW.
-      eexists. apply (Rule_Abs). reflexivity. apply H.
-      Unshelve. apply update_compatible. assumption.
-    * apply well_typed_Choice in HW. destruct HW as [HW1 HW2].
-      destruct (IHe1 Rho Gamma HG HW1).
-      destruct (IHe2 Rho Gamma HG HW2).
-      exists ND. eapply Rule_Choice. apply H. apply H0.
-    * destruct b.
-      - remember HW as HWC. clear HeqHWC.
-        apply well_typed_Case_Unit in HW. destruct HW as [HW1 HW2].
-        destruct (IHe Rho Gamma HG HW1).
-        destruct (completeness e0 Rho Gamma HG HW2).
-        destruct x.
-        + exists x0. eapply Rule_CaseDUnit. apply H. apply H0.
-        + exists ND. eapply Rule_CaseNDUnit. apply H. apply H0.
-        + destruct (compatibility e Rho Gamma (Arrow x1 x2) HG HW1 H).
-          destruct H1.
-          unfold well_typed in HWC.
-          unfold typeOf in HWC. fold typeOf in HWC.
-          rewrite H1 in HWC.
-          destruct x; inversion H2. inversion HWC.
-      - destruct p.
-        remember HW as HWC. clear HeqHWC.
-        apply well_typed_Case_Pair in HW. destruct HW as [HW1 HW2].
-        destruct (IHe Rho Gamma HG HW1).
-        edestruct (completeness e0).
-        reflexivity. apply HW2.
-        destruct x.
-        + exists x0. eapply Rule_CaseDPair.
-          apply H. erewrite update_update_compatible.
-          apply H0. apply HG.
-        + exists ND. eapply Rule_CaseNDPair. apply H.
-          erewrite update_update_compatible.
-          apply H0. apply HG.
-        + destruct (compatibility e Rho Gamma (Arrow x1 x2) HG HW1 H).
-          destruct H1.
-          unfold well_typed in HWC.
-          unfold typeOf in HWC. fold typeOf in HWC.
-          rewrite H1 in HWC.
-          destruct x; inversion H2. inversion HWC.
+      - eapply compatibility in H. shelve.
+        eassumption. apply Heq1. Unshelve. inversion H.
+      - exists ND. split. eapply Rule_AppND. apply H. apply H3.
+        reflexivity.
+      - eexists. split. eapply Rule_AppFun. apply H. apply H3.
+        reflexivity. simpl in H2. destruct H2.
+        unfold decide. destruct (more_specific x0 x1) eqn:Heq4.
+        assumption. reflexivity.
+    * unfold typeOf in HW. fold typeOf in HW.
+      destruct (typeOf (update Nat.eqb Rho n t) e) eqn:Heq1;
+      try inversion HW; subst.
+      edestruct (IHe (update Nat.eqb Rho n t)).
+      shelve. apply Heq1. destruct H.
+      eexists. split. apply (Rule_Abs). shelve. apply H.
+      simpl. split. apply mkCompatible_compatible. apply H0.
+      Unshelve. unfold compatibleCtx in *. intros n0.
+      unfold update. destruct (Nat.eqb n n0) eqn:Heq2.
+      apply mkCompatible_compatible. apply HG.
+      apply mkCompatible_compatible.
+    * unfold typeOf in HW. fold typeOf in HW.
+      destruct (typeOf Rho e1) eqn:Heq1, (typeOf Rho e2) eqn:Heq2;
+      try inversion HW; subst.
+      destruct (eqType t t1) eqn:Heq3; try inversion H0; subst.
+      apply eq_Type_eq in Heq3. subst.
+      destruct (IHe1 Rho Gamma t1 HG Heq1). destruct H.
+      destruct (IHe2 Rho Gamma t1 HG Heq2). destruct H2.
+      exists ND. split. eapply Rule_Choice. apply H. apply H2.
+      reflexivity.
+    * simpl in HW.
+      destruct (typeOf Rho e1) eqn:Heq1;
+      try discriminate; destruct t;
+      destruct (typeOf Rho e2) eqn:Heq2;
+      destruct (typeOf Rho e3) eqn:Heq3;
+      try discriminate;
+      destruct (eqType t t1) eqn:Heq4;
+      try discriminate; apply eq_Type_eq in Heq4;
+      inversion HW; subst.
+      destruct (IHe1 _ _ _ HG Heq1). destruct H.
+      destruct (IHe2 _ _ _ HG Heq2). destruct H1.
+      destruct (IHe3 _ _ _ HG Heq3). destruct H3.
+      exists (lub x x0 x1). split.
+      eapply Rule_CaseBool; try eassumption.
+      apply compatible_lub; try assumption.
+    * simpl in HW. destruct p.
+      destruct (typeOf Rho e1) eqn:Heq1;
+      try discriminate. simpl in HW.
+      destruct (eqType t (TList t1)) eqn:Heq4;
+      try discriminate. apply eq_Type_eq in Heq4; subst.
+      destruct (typeOf Rho e2) eqn:Heq2;
+      try discriminate;
+      destruct (typeOf (update Nat.eqb
+                  (update Nat.eqb Rho n2 (TList t1))
+                  n1 t1) e3)eqn:Heq3;
+      try discriminate. simpl in HW.
+      destruct (eqType t t2) eqn:Heq5;
+      try discriminate; apply eq_Type_eq in Heq5;
+      inversion HW; subst.
+      destruct (IHe1 _ _ _ HG Heq1). destruct H.
+      destruct (IHe2 _ _ _ HG Heq2). destruct H1.
+      eapply IHe3 in Heq3. destruct Heq3, H3.
+      exists (lub x x0 x1). split.
+      eapply Rule_CaseList; try eassumption.
+      shelve. apply compatible_lub; try assumption.
+      destruct x; inversion H0; reflexivity.
+      rewrite double_update_indep.
+      apply update_compatible.
+      apply update_compatible.
+      assumption. assumption. shelve.
+      assumption. Unshelve. apply ND.
+      reflexivity. reflexivity.
   Qed.
 
-  Lemma hasDType_unbound : forall e Gamma d t n,
-    Gamma |- e ::: d ->
+  Lemma hasDType_unbound : forall e Gamma d1 d2 n,
+    Gamma |- e ::: d1 ->
     anyIn (freeVars e) [n] = false ->
-    update Nat.eqb Gamma n (mkCompatible t) |- e ::: d.
+    update Nat.eqb Gamma n d2 |- e ::: d1.
   Proof.
     fix hasDType_unbound 1.
     induction e; intros.
@@ -1902,14 +2101,20 @@ Section Proofs.
       + subst. apply Rule_Var. unfold update. rewrite Heq.
         inversion H. assumption.
     - inversion H. subst. simpl in *.
-      apply Rule_Unit. reflexivity.
+      apply Rule_BTrue.
+    - inversion H. subst. simpl in *.
+      apply Rule_BFalse.
+    - inversion H. subst. simpl in *.
+      apply Rule_Nil.
     - inversion H. subst. simpl in *.
       apply anyIn_cons in H0. destruct H0 as [HH1 HH2].
       apply anyIn_concat2 in HH1. destruct HH1 as [HH3 HH4].
       apply anyIn_concat2 in HH2. destruct HH2 as [HH5 HH6].
-      eapply IHe1 in H3. eapply IHe2 in H5.
-      eapply Rule_Pair. eassumption. eassumption. reflexivity.
-      eassumption. eassumption.
+      destruct d0 eqn:HeqD0, d3 eqn:HeqD3;
+      eapply Rule_Cons with (d1 := d0) (d2 := d3); subst;
+      try apply (IHe1 Gamma _ _ n); try eassumption;
+      try apply (IHe2 Gamma _ _ n); try eassumption;
+      try reflexivity.
     - unfold freeVars in H0. fold freeVars in H0.
       apply anyIn_concat2 in H0. destruct H0 as [H0_1 H0_2].
       inversion H; subst; simpl in *.
@@ -1922,10 +2127,10 @@ Section Proofs.
     - inversion H. subst. simpl in *.
       destruct (n0 =? n) eqn:Heq.
       + rewrite Nat.eqb_eq in Heq. subst.
-        eapply Rule_Abs. reflexivity.
+        eapply Rule_Abs. assumption.
         rewrite double_update. eassumption.
       + apply Nat.eqb_neq in Heq. eapply IHe in H7.
-        eapply Rule_Abs. reflexivity. rewrite double_update_indep.
+        eapply Rule_Abs. assumption. rewrite double_update_indep.
         apply H7. assumption. apply anyIn_removeb in H0. assumption.
         symmetry. assumption.
     - inversion H. subst. simpl in *.
@@ -1933,75 +2138,56 @@ Section Proofs.
       eapply IHe1 in H4. eapply IHe2 in H6.
       eapply Rule_Choice. eassumption. eassumption.
       assumption. assumption.
-    - destruct b eqn:HeqB; inversion H; subst; simpl in *.
-      + apply anyIn_concat2 in H0. destruct H0 as [H0_1 H0_2].
-        eapply IHe in H0_1.
-        apply (hasDType_unbound e0 Gamma d0 t) in H0_2.
-        eapply Rule_CaseNDUnit. eassumption. eassumption.
-        eassumption. eassumption.
-      + apply anyIn_concat2 in H0. destruct H0 as [H0_1 H0_2].
-        eapply IHe in H0_1.
-        apply (hasDType_unbound e0 Gamma d t) in H0_2.
-        eapply Rule_CaseDUnit. eassumption. eassumption.
-        eassumption. eassumption.
-      + subst p0. apply anyIn_concat2 in H0. destruct H0 as [H0_1 H0_2].
-        subst Gamma''. subst Gamma'.
-        destruct (n1 =? n) eqn:Heq1, (n2 =? n) eqn:Heq2.
-        * apply Nat.eqb_eq in Heq1. subst.
-          eapply IHe in H0_1. eapply Rule_CaseNDPair.
-          eassumption. rewrite double_update. apply H8.
-          apply H7.
-        * apply Nat.eqb_eq in Heq1. apply Nat.eqb_neq in Heq2. subst.
-          eapply IHe in H0_1. eapply Rule_CaseNDPair.
-          eassumption. rewrite double_update. apply H8.
-          apply H7.
-        * apply Nat.eqb_neq in Heq1. apply Nat.eqb_eq in Heq2. subst.
-          eapply IHe in H0_1. eapply Rule_CaseNDPair.
-          eassumption. rewrite double_update_indep.
-          rewrite double_update. rewrite double_update_indep.
-          apply H8. symmetry. assumption. assumption. assumption.
-        * apply Nat.eqb_neq in Heq1. apply Nat.eqb_neq in Heq2.
-          eapply IHe in H0_1. eapply anyIn_removeb in H0_2.
-          eapply anyIn_removeb in H0_2.
-          apply (hasDType_unbound e0
-                   (update Nat.eqb (update Nat.eqb Gamma n1
-                           (mkCompatible t1))n2 (mkCompatible t2)) d0 t)
-                     in H0_2.
-          eapply Rule_CaseNDPair.
-          eassumption.
-          rewrite (double_update_indep _ n _ n1).
-          rewrite (double_update_indep _ n _ n2).
-          apply H0_2. symmetry. eassumption. symmetry. eassumption.
-          apply H8. eassumption. eassumption. eassumption.
-      + subst p0. apply anyIn_concat2 in H0. destruct H0 as [H0_1 H0_2].
-        subst Gamma''. subst Gamma'.
-        destruct (n1 =? n) eqn:Heq1, (n2 =? n) eqn:Heq2.
-        * apply Nat.eqb_eq in Heq1. subst.
-          eapply IHe in H0_1. eapply Rule_CaseDPair.
-          eassumption. rewrite double_update. apply H8.
-          apply H7.
-        * apply Nat.eqb_eq in Heq1. apply Nat.eqb_neq in Heq2. subst.
-          eapply IHe in H0_1. eapply Rule_CaseDPair.
-          eassumption. rewrite double_update. apply H8.
-          apply H7.
-        * apply Nat.eqb_neq in Heq1. apply Nat.eqb_eq in Heq2. subst.
-          eapply IHe in H0_1. eapply Rule_CaseDPair.
-          eassumption. rewrite double_update_indep.
-          rewrite double_update. rewrite double_update_indep.
-          apply H8. symmetry. assumption. assumption. assumption.
-        * apply Nat.eqb_neq in Heq1. apply Nat.eqb_neq in Heq2.
-          eapply IHe in H0_1. eapply anyIn_removeb in H0_2.
-          eapply anyIn_removeb in H0_2.
-          apply (hasDType_unbound e0
-                   (update Nat.eqb (update Nat.eqb Gamma n1
-                           (mkCompatible t1))n2 (mkCompatible t2)) d t)
-                     in H0_2.
-          eapply Rule_CaseDPair.
-          eassumption.
-          rewrite (double_update_indep _ n _ n1).
-          rewrite (double_update_indep _ n _ n2).
-          apply H0_2. symmetry. eassumption. symmetry. eassumption.
-          apply H8. eassumption. eassumption. eassumption.
+    - inversion H. subst. simpl in *.
+      apply anyIn_concat2 in H0.
+      destruct H0 as [HH1 HH2].
+      apply anyIn_concat2 in HH2.
+      destruct HH2 as [HH3 HH4].
+      apply Rule_CaseBool.
+      apply IHe1; assumption.
+      apply IHe2; assumption.
+      apply IHe3; assumption.
+    - inversion H. subst. simpl in *.
+      apply anyIn_concat2 in H0.
+      destruct H0 as [HH1 HH2].
+      apply anyIn_concat2 in HH2.
+      destruct HH2 as [HH3 HH4].
+      eapply Rule_CaseList.
+      apply IHe1; assumption. apply H8. apply H10.
+      apply IHe2; assumption.
+      destruct (n =? n2) eqn:HeqN2,
+               (n =? n1) eqn:HeqN1.
+      + apply Nat.eqb_eq in HeqN2.
+        apply Nat.eqb_eq in HeqN1. subst.
+        rewrite double_update.
+        rewrite double_update.
+        subst Gamma'. subst Gamma''.
+        rewrite double_update in H12.
+        assumption.
+      + apply Nat.eqb_eq in HeqN2.
+        apply Nat.eqb_neq in HeqN1. subst.
+        rewrite double_update_indep.
+        rewrite double_update.
+        subst Gamma'. subst Gamma''.
+        rewrite double_update_indep in H12.
+        assumption. symmetry. assumption.
+        symmetry. assumption.
+      + apply Nat.eqb_neq in HeqN2.
+        apply Nat.eqb_eq in HeqN1. subst.
+        rewrite double_update.
+        subst Gamma'. subst Gamma''.
+        assumption.
+      + apply Nat.eqb_neq in HeqN2.
+        apply Nat.eqb_neq in HeqN1. subst.
+        rewrite (double_update_indep _ n _ n1).
+        rewrite (double_update_indep _ n _ n2).
+        subst Gamma'. subst Gamma''.
+        apply anyIn_removeb in HH4.
+        apply anyIn_removeb in HH4.
+        apply IHe3; assumption.
+        symmetry. assumption.
+        symmetry. assumption.
+        assumption. assumption.
   Qed.
 
   (* Lemma subst_lemma:
@@ -2009,12 +2195,12 @@ Section Proofs.
    determinism type d2, and we substitute a well-typed expression e2 with
    compatible determinism type, then the result maintains a determinism type
    that is at least as specific as the original. *)
-  Lemma subst_lemma : forall e1 e2 Rho t1 d2 d3 n,
+  Lemma subst_lemma : forall e1 e2 Rho Gamma t1 d1 d2 d3 n,
     anyIn (freeVars e2) (n::boundVars e1) = false ->
     well_typed (update Nat.eqb Rho n t1) e1 ->
     typeOf Rho e2 = Some t1 ->
-    let Gamma := mkCompatibleCtx Rho in
-    let d1 := mkCompatible t1 in
+    compatibleCtx Gamma Rho ->
+    compatible d1 t1 ->
     update Nat.eqb Gamma n d1 |- e1 ::: d2 ->
     more_specific d3 d1 = true ->
     Gamma |- e2 ::: d3 ->
@@ -2022,9 +2208,8 @@ Section Proofs.
       more_specific d4 d2 = true /\
       Gamma |- subst n e2 e1 ::: d4.
   Proof.
-    fix subst_lemma 1.
-    --
-    induction e1; intros.
+    induction e1; intro;
+    intros Rho Gamma t1 d1 d2 d3 n0 H H0 H1 H3 H4; intros.
     - inversion H2. subst. simpl.
       unfold update. destruct (Nat.eqb n n0) eqn:Heq.
       + apply Nat.eqb_eq in Heq. subst.
@@ -2037,20 +2222,27 @@ Section Proofs.
         apply Rule_Var. reflexivity.
     - inversion H2. subst. simpl in *.
       exists D. split. apply more_specific_refl.
-      apply Rule_Unit. reflexivity.
+      apply Rule_BTrue.
+    - inversion H2. subst. simpl in *.
+      exists D. split. apply more_specific_refl.
+      apply Rule_BFalse.
+    - inversion H2. subst. simpl in *.
+      exists D. split. apply more_specific_refl.
+      apply Rule_Nil.
     - inversion H2. subst. simpl in *.
       apply anyIn_cons in H. destruct H as [HH1 HH2].
       apply anyIn_concat1 in HH1. destruct HH1 as [HH3 HH4].
-      apply well_typed_Pair in H0. destruct H0 as [H0_1 H0_2].
-      edestruct IHe1_1 in H7. apply anyIn_cons_r; eassumption. eassumption. eassumption. eassumption. eassumption.
-      eassumption.
-      edestruct IHe1_2 in H9. apply anyIn_cons_r; eassumption.
+      apply well_typed_Cons in H0. destruct H0 as [H0_1 H0_2].
+      edestruct IHe1_1 in H9. apply anyIn_cons_r; eassumption. eassumption. eassumption. eassumption. eassumption.
+      eassumption. apply H5. apply H6.
+      edestruct IHe1_2 in H11. apply anyIn_cons_r; eassumption.
       eassumption. eassumption. eassumption. eassumption.
-      eassumption. destruct H. destruct H0. eexists. split.
-      shelve. eapply Rule_Pair. eassumption. eassumption.
-      reflexivity. Unshelve. subst d1.
+      eassumption. apply H5. apply H6.
+      destruct H, H0. eexists. split.
+      shelve. eapply Rule_Cons. eassumption. eassumption.
+      reflexivity. Unshelve.
       destruct x, x0, d0, d4; try inversion H;
-      try inversion H0; try rewrite H10; try reflexivity.
+      try inversion H0; try rewrite H12; try reflexivity.
     - remember H0 as HWC. clear HeqHWC.
       apply well_typed_App in H0. destruct H0 as [H0_1 H0_2].
       apply anyIn_cons in H. destruct H as [HH1 HH2].
@@ -2060,7 +2252,7 @@ Section Proofs.
         edestruct IHe1_1 in H6; try apply anyIn_cons_r; try eassumption.
         edestruct IHe1_2 in H8; try apply anyIn_cons_r; try eassumption.
         destruct H. destruct H0. eapply Rule_AppND.
-        apply H5. apply H7.
+        apply H7. apply H9.
       + remember H4 as H4C. clear HeqH4C.
         edestruct IHe1_1 in H5; try apply anyIn_cons_r; try eassumption.
         edestruct IHe1_2 in H7; try apply anyIn_cons_r; try eassumption.
@@ -2068,7 +2260,7 @@ Section Proofs.
         * inversion H.
         * inversion H.
         * eexists. split. shelve.
-          eapply Rule_AppFun. apply H6. apply H8. reflexivity.
+          eapply Rule_AppFun. apply H8. apply H10. reflexivity.
           Unshelve. simpl in H. apply andb_true_iff in H.
           destruct H. unfold decide.
           destruct (more_specific d5 d0) eqn:Heq1.
@@ -2082,286 +2274,222 @@ Section Proofs.
       apply anyIn_cons in H. destruct H as [HH1 HH2].
       apply anyIn_Abs in HH1. destruct HH1 as [HH3 HH4].
       destruct (n0 =? n) eqn:Heq.
-      + subst d1. apply Nat.eqb_eq in Heq. subst.
+      + apply Nat.eqb_eq in Heq. subst.
         eexists. simpl. rewrite Nat.eqb_refl.
-        split. shelve. eapply Rule_Abs.
-        reflexivity. subst Gamma'.
-        rewrite double_update in H11. apply H11.
+        split. shelve. eapply Rule_Abs. apply H12.
+        subst Gamma'. rewrite double_update in H13. apply H13.
         Unshelve. simpl. rewrite less_specific_refl. rewrite more_specific_refl. reflexivity.
       + apply Nat.eqb_neq in Heq. subst Gamma'.
         rewrite double_update_indep in H0; try assumption.
-        rewrite double_update_indep in H11; try assumption.
-        edestruct IHe1 in H11. apply anyIn_cons_r; eassumption.
-        eassumption. erewrite typeOf_unbound. eassumption. eassumption.
-        eassumption. erewrite update_compatible. subst d1.
-        erewrite update_update_compatible in H11. apply H11.
-        reflexivity. reflexivity. subst Gamma. apply H3.
-        erewrite <- update_compatible.
-        apply hasDType_unbound. apply H4. assumption.
-        reflexivity. destruct H. eexists. split. shelve. simpl.
+        rewrite double_update_indep in H13; try assumption.
+        edestruct IHe1 in H13. apply anyIn_cons_r; eassumption.
+        eassumption. erewrite typeOf_unbound. eassumption. eassumption. eassumption. shelve.
+        eassumption. apply H13. eassumption.
+        apply hasDType_unbound. apply H6. assumption.
+        destruct H. eexists. split. shelve. simpl.
         apply Nat.eqb_neq in Heq. rewrite Nat.eqb_sym in Heq.
-        rewrite Heq. eapply Rule_Abs. reflexivity.
-        erewrite update_compatible. apply H5. reflexivity.
-        Unshelve. simpl. rewrite less_specific_refl.
+        rewrite Heq. eapply Rule_Abs. apply H12. apply H7.
+        Unshelve. apply update_compatible; assumption.
+        simpl. rewrite less_specific_refl.
         rewrite H. reflexivity.
     - inversion H2. subst.
       apply well_typed_Choice in H0. destruct H0 as [H0_1 H0_2].
       apply anyIn_cons in H. destruct H as [HH1 HH2].
       apply anyIn_concat1 in HH1. destruct HH1 as [HH3 HH4].
-      edestruct IHe1_1 in H8. apply anyIn_cons_r; eassumption.
-      eassumption. eassumption. eassumption. eassumption. eassumption.
+      edestruct IHe1_1 in H10. apply anyIn_cons_r; eassumption.
+      eassumption. eassumption. eassumption. eassumption. eassumption. eassumption. eassumption.
       edestruct IHe1_2 in H10. apply anyIn_cons_r; eassumption.
-      eassumption. eassumption. eassumption. eassumption. eassumption.
+      eassumption. eassumption. eassumption. eassumption. eassumption. eassumption. eassumption.
       destruct H, H0.
       exists ND. split. apply more_specific_ND. simpl.
       eapply Rule_Choice; eassumption.
-    - destruct b; inversion H2; subst.
-      * remember H0 as H0C. clear HeqH0C.
-        apply well_typed_Case_Unit in H0.
-        destruct H0 as [H0A H0B].
-        apply anyIn_cons in H. destruct H as [HH1 HH2].
-        apply anyIn_Case_Unit in HH1. destruct HH1 as [HH3 HH4].
-        edestruct IHe1 in H0A. apply anyIn_cons_r; eassumption.
-        eassumption. eassumption. eassumption. apply H3. eassumption.
-        edestruct subst_lemma. apply anyIn_cons_r. apply HH4.
-        eassumption. eassumption. eassumption. eassumption.
-        eassumption. eassumption. destruct H, H0. destruct x.
-        + exists x0. split. apply more_specific_ND. simpl.
-          apply Rule_CaseDUnit. assumption. assumption.
-        + exists ND. split. apply more_specific_ND. simpl.
-          eapply Rule_CaseNDUnit. assumption. eassumption.
-        + unfold well_typed in H0A. unfold well_typed in H0B.
-          destruct (typeOf (update Nat.eqb Rho n t1) e1) eqn:Heq1;
-          destruct (typeOf (update Nat.eqb Rho n t1) e) eqn:Heq2;
-          try contradiction.
-          eapply subst_preservation in H1. shelve.
-          apply anyIn_cons_r. apply HH3. apply HH2. apply Heq1.
-          Unshelve. edestruct compatibility. reflexivity.
-          unfold well_typed. rewrite H1. reflexivity.
-          apply H5. destruct H7. rewrite H1 in H7. inversion H7.
-          subst. unfold well_typed in H0C. unfold typeOf in H0C.
-          fold typeOf in H0C. rewrite Heq1 in H0C.
-          destruct x; try inversion H9; contradiction.
-      * remember H0 as H0C. clear HeqH0C.
-        apply well_typed_Case_Unit in H0.
-        destruct H0 as [H0A H0B].
-        apply anyIn_cons in H. destruct H as [HH1 HH2].
-        apply anyIn_Case_Unit in HH1. destruct HH1 as [HH3 HH4].
-        edestruct IHe1 in H0A. apply anyIn_cons_r; eassumption.
-        eassumption. eassumption. eassumption. apply H3. eassumption.
-        edestruct subst_lemma. apply anyIn_cons_r. apply HH4.
-        eassumption. eassumption. eassumption. eassumption.
-        eassumption. eassumption. destruct H, H0. destruct x.
-        + exists x0. split. assumption. simpl.
-          apply Rule_CaseDUnit. assumption. assumption.
-        + inversion H.
-        + unfold well_typed in H0A. unfold well_typed in H0B.
-          destruct (typeOf (update Nat.eqb Rho n t1) e1) eqn:Heq1;
-          destruct (typeOf (update Nat.eqb Rho n t1) e) eqn:Heq2;
-          try contradiction.
-          eapply subst_preservation in H1. shelve.
-          apply anyIn_cons_r. apply HH3. apply HH2. apply Heq1.
-          Unshelve. edestruct compatibility. reflexivity.
-          unfold well_typed. rewrite H1. reflexivity.
-          apply H5. destruct H7. rewrite H1 in H7. inversion H7.
-          subst. unfold well_typed in H0C. unfold typeOf in H0C.
-          fold typeOf in H0C. rewrite Heq1 in H0C.
-          destruct x; try inversion H9; contradiction.
-      * remember H0 as H0C. clear HeqH0C.
-        apply well_typed_Case_Pair in H0.
-        destruct H0 as [H0A H0B].
-        remember H12 as H12C. clear HeqH12C.
-        apply anyIn_cons in H. destruct H as [HH1 HH2].
-        apply anyIn_Case_Pair in HH1. destruct HH1 as [HH3 HH4].
-        apply anyIn_cons in HH4. destruct HH4 as [HH5 HH6].
-        apply anyIn_cons in HH5. destruct HH5 as [HH7 HH8].
-        edestruct IHe1 in H0A. apply anyIn_cons_r; eassumption.
-        eassumption. eassumption. eassumption. apply H3. eassumption.
-        destruct H. simpl.
-        destruct (n =? n1) eqn:Heq1, (n =? n2) eqn:Heq2.
-        + apply Nat.eqb_eq in Heq1. apply Nat.eqb_eq in Heq2. subst.
-          subst Gamma''. subst Gamma'.
-          erewrite double_update in H12. erewrite double_update in H12.
-          destruct x.
-          ++  exists d. split. apply more_specific_ND.
-              apply Rule_CaseDPair. assumption.
-              erewrite double_update. apply H12.
-          ++  exists ND. split. apply more_specific_ND. simpl.
-              eapply Rule_CaseNDPair. assumption.
-              erewrite double_update. eassumption.
-          ++  unfold well_typed in H0A. unfold well_typed in H0B.
-              destruct (typeOf (update Nat.eqb Rho n2 t1) e1) eqn:Heq1;
-              destruct (typeOf (update Nat.eqb Rho n2 t1) e) eqn:Heq2;
-              try contradiction.
-        + apply Nat.eqb_eq in Heq1. apply Nat.eqb_neq in Heq2. subst.
-          subst Gamma''. subst Gamma'.
-          erewrite double_update in H12.
-          erewrite double_update_indep in H12. shelve. assumption.
-          Unshelve. destruct x.
-          ++  exists d. split. apply more_specific_ND.
-              apply Rule_CaseDPair. assumption.
-              erewrite double_update_indep. apply H12. assumption.
-          ++  exists ND. split. apply more_specific_ND. simpl.
-              eapply Rule_CaseNDPair. assumption.
-              erewrite double_update_indep. eassumption. eassumption.
-          ++  unfold well_typed in H0A. unfold well_typed in H0B.
-              destruct (typeOf (update Nat.eqb Rho n1 t1) e1) eqn:Heq4;
-              try contradiction.
-              eapply subst_preservation in H1. shelve.
-              apply anyIn_cons_r. apply HH3. apply HH2. apply Heq4.
-              Unshelve. edestruct compatibility. reflexivity.
-              unfold well_typed. rewrite H1. reflexivity. apply H0.
-              destruct p0. subst. unfold well_typed in H0C.
-              unfold typeOf in H0C. fold typeOf in H0C.
-              rewrite Heq4 in H0C. destruct t; try contradiction.
-              destruct H6. rewrite H1 in H6. inversion H6. subst.
-              inversion H7.
-        + apply Nat.eqb_neq in Heq1. apply Nat.eqb_eq in Heq2. subst.
-          subst Gamma''. subst Gamma'.
-          erewrite double_update_indep in H12.
-          erewrite double_update in H12.  shelve. assumption.
-          Unshelve. destruct x.
-          ++  exists d. split. apply more_specific_ND.
-              apply Rule_CaseDPair. assumption.
-              erewrite double_update_indep. apply H12. assumption.
-          ++  exists ND. split. apply more_specific_ND. simpl.
-              eapply Rule_CaseNDPair. assumption.
-              erewrite double_update_indep. eassumption. eassumption.
-          ++  unfold well_typed in H0A. unfold well_typed in H0B.
-              destruct (typeOf (update Nat.eqb Rho n2 t1) e1) eqn:Heq4;
-              try contradiction.
-              eapply subst_preservation in H1. shelve.
-              apply anyIn_cons_r. apply HH3. apply HH2. apply Heq4.
-              Unshelve. edestruct compatibility. reflexivity.
-              unfold well_typed. rewrite H1. reflexivity. apply H0.
-              destruct p0. subst. unfold well_typed in H0C.
-              unfold typeOf in H0C. fold typeOf in H0C.
-              rewrite Heq4 in H0C. destruct t; try contradiction.
-              destruct H6. rewrite H1 in H6. inversion H6. subst.
-              inversion H7.
-        + apply Nat.eqb_neq in Heq1. apply Nat.eqb_neq in Heq2.
-          subst Gamma''. subst Gamma'. simpl.
-          rewrite (double_update_indep _ n _ n1) in H0B.
-          rewrite (double_update_indep _ n _ n2) in H0B.
-          shelve. assumption. assumption. Unshelve.
-          edestruct subst_lemma. apply anyIn_cons_r. apply HH7.
-          eassumption. eassumption.
-          erewrite typeOf_unbound. erewrite typeOf_unbound.
-          apply H1. apply H1. assumption.
-          erewrite typeOf_unbound. eassumption. eassumption.
-          eassumption. eassumption.
-          erewrite <- update_compatible.
-          rewrite (double_update_indep _ n _ n1) in H12.
-          rewrite (double_update_indep _ n _ n2) in H12.
-          apply H12. assumption. assumption.
-          apply update_compatible. reflexivity. apply H3.
-          erewrite <- update_compatible with
-            (Gamma := mkCompatibleCtx (update Nat.eqb Rho n1 t0)).
-          erewrite <- update_compatible with
-            (Gamma := mkCompatibleCtx Rho).
-          eapply hasDType_unbound.
-          eapply hasDType_unbound.
-          apply H4. assumption. assumption. reflexivity. reflexivity.
-          destruct H6. destruct x.
-          ++  exists x0. split. apply more_specific_ND.
-              apply Rule_CaseDPair. assumption.
-              erewrite update_compatible. apply H7.
-              apply update_compatible. reflexivity.
-          ++  exists ND. split. apply more_specific_ND. simpl.
-              eapply Rule_CaseNDPair. assumption.
-              erewrite update_compatible. apply H7.
-              apply update_compatible. reflexivity.
-          ++  unfold well_typed in H0A. unfold well_typed in H0B.
-              destruct (typeOf (update Nat.eqb Rho n t1) e1) eqn:Heq3;
-              try contradiction.
-              destruct (typeOf (update Nat.eqb (update Nat.eqb
-                               (update Nat.eqb Rho n1 t0) n2 t2)
-                                n t1) e) eqn:Heq4;
-              try contradiction.
-              eapply subst_preservation in H1. shelve.
-              apply anyIn_cons_r. apply HH3. apply HH2. apply Heq3.
-              Unshelve. edestruct compatibility. reflexivity.
-              unfold well_typed. rewrite H1. reflexivity. apply H0.
-              destruct p0. subst. unfold well_typed in H0C.
-              unfold typeOf in H0C. fold typeOf in H0C.
-              rewrite Heq3 in H0C. destruct t; try contradiction.
-              destruct H8. rewrite H1 in H8. inversion H8. subst.
-              inversion H9.
-    * remember H0 as H0C. clear HeqH0C.
-      apply well_typed_Case_Pair in H0.
-      destruct H0 as [H0A H0B].
-      remember H12 as H12C. clear HeqH12C.
+    - inversion H2. subst.
+      remember H0 as HC. clear HeqHC.
+      apply well_typed_CaseB in H0.
+      destruct H0 as [H0_1 [H0_2 H0_3]].
       apply anyIn_cons in H. destruct H as [HH1 HH2].
-      apply anyIn_Case_Pair in HH1. destruct HH1 as [HH3 HH4].
-      apply anyIn_cons in HH4. destruct HH4 as [HH5 HH6].
-      apply anyIn_cons in HH5. destruct HH5 as [HH7 HH8].
-      edestruct IHe1 in H0A. apply anyIn_cons_r; eassumption.
-      eassumption. eassumption. eassumption. apply H3. eassumption.
-      destruct H. simpl.
-      destruct (n =? n1) eqn:Heq1, (n =? n2) eqn:Heq2.
-      + apply Nat.eqb_eq in Heq1. apply Nat.eqb_eq in Heq2. subst.
-        subst Gamma''. subst Gamma'.
-        erewrite double_update in H12. erewrite double_update in H12.
-        destruct x.
-        ++  exists d2. split. apply more_specific_refl.
-            apply Rule_CaseDPair. assumption.
-            erewrite double_update. apply H12.
-        ++  inversion H.
-        ++  inversion H.
-      + apply Nat.eqb_eq in Heq1. apply Nat.eqb_neq in Heq2. subst.
-        subst Gamma''. subst Gamma'.
-        erewrite double_update in H12.
-        erewrite double_update_indep in H12. shelve. assumption.
-        Unshelve. destruct x.
-        ++  exists d2. split. apply more_specific_refl.
-            apply Rule_CaseDPair. assumption.
-            erewrite double_update_indep. apply H12. assumption.
-        ++  inversion H.
-        ++  inversion H.
-      + apply Nat.eqb_neq in Heq1. apply Nat.eqb_eq in Heq2. subst.
-        subst Gamma''. subst Gamma'.
-        erewrite double_update_indep in H12.
-        erewrite double_update in H12.  shelve. assumption.
-        Unshelve. destruct x.
-        ++  exists d2. split. apply more_specific_refl.
-            apply Rule_CaseDPair. assumption.
-            erewrite double_update_indep. apply H12. assumption.
-        ++  inversion H.
-        ++  inversion H.
-      + apply Nat.eqb_neq in Heq1. apply Nat.eqb_neq in Heq2.
-        subst Gamma''. subst Gamma'. simpl.
-        rewrite (double_update_indep _ n _ n1) in H0B.
-        rewrite (double_update_indep _ n _ n2) in H0B.
-        shelve. assumption. assumption. Unshelve.
-        edestruct subst_lemma. apply anyIn_cons_r. apply HH7.
+      apply anyIn_Case_Bool in HH1.
+      destruct HH1 as [HH3 [HH4 HH5]].
+      edestruct IHe1_1 in H0_1.
+      apply anyIn_cons_r; eassumption.
+      eassumption. eassumption. eassumption.
+      eassumption. eassumption. eassumption.
+      eassumption. destruct H.
+      edestruct IHe1_2 in H0_2.
+      apply anyIn_cons_r; eassumption.
+      eassumption. eassumption. eassumption.
+      eassumption. eassumption. eassumption.
+      eassumption. destruct H7.
+      edestruct IHe1_3 in H0_3.
+      apply anyIn_cons_r; eassumption.
+      eassumption. eassumption. eassumption.
+      eassumption. eassumption. eassumption.
+      eassumption. destruct H9.
+      exists (lub x x0 x1). split.
+      * apply more_specific_lub; try assumption.
+        unfold well_typed in HC. simpl in HC.
+        destruct (typeOf (update Nat.eqb Rho n0 t1)
+                   e1_1) eqn:Heq1;
+        try inversion HC. destruct t;
+        try inversion HC.
+        remember Heq1 as Heq1C. clear HeqHeq1C.
+        eapply compatibility in Heq1. shelve.
+        shelve. apply H11. Unshelve.
+        -- eapply subst_preservation in H1.
+           shelve. shelve. apply Heq1C.
+           Unshelve.
+           eapply compatibility in H1. apply H1.
+           eassumption. eassumption.
+           apply anyIn_cons_r; assumption.
+        -- apply update_compatible.
+           assumption. assumption.
+      * simpl. apply Rule_CaseBool; assumption.
+    - inversion H2. subst.
+      remember H0 as HC. clear HeqHC.
+      apply well_typed_CaseL in H0.
+      destruct H0 as [H0_1 [H0_2 H0_3]].
+      apply anyIn_cons in H. destruct H as [HH1 HH2].
+      apply anyIn_Case_List in HH1.
+      destruct HH1 as [HH3 [HH4 HH5]].
+      apply anyIn_cons in HH5.
+      destruct HH5 as [HH6 HH7].
+      apply anyIn_cons in HH6.
+      destruct HH6 as [HH8 HH9].
+      unfold well_typed in HC.
+      simpl in HC.
+      remember (update Nat.eqb Rho n0 t1) as Rho'.
+      destruct (typeOf Rho' e1_1) eqn:Heq1;
+      try inversion HC. simpl in HC.
+      destruct (eqType t (TList t0)) eqn:Heq2;
+      try inversion HC; apply eq_Type_eq in Heq2.
+      destruct (typeOf Rho' e1_2) eqn:Heq3,
+                (typeOf (update Nat.eqb
+                        (update Nat.eqb Rho' n2
+                        (TList t0)) n1 t0) e1_3)
+          eqn:Heq4;
+      try inversion HC; simpl in HC.
+      destruct (eqType t2 t3) eqn:Heq5;
+      try inversion HC; apply eq_Type_eq in Heq5; subst.
+      edestruct IHe1_1 in H0_1.
+      apply anyIn_cons_r; try eassumption.
+      eassumption. eassumption. eassumption.
+      eassumption. eassumption. eassumption.
+      eassumption. destruct H.
+      edestruct IHe1_2 in H0_2.
+      apply anyIn_cons_r; try eassumption.
+      eassumption. eassumption. eassumption.
+      eassumption. eassumption. eassumption. eassumption.
+      destruct H8.
+      destruct (Nat.eqb n0 n1) eqn:HeqN1,
+               (Nat.eqb n0 n2) eqn:HeqN2.
+      + rewrite Nat.eqb_eq in HeqN1. subst n1.
+        rewrite Nat.eqb_eq in HeqN2. subst n2.
+        contradiction.
+      + rewrite Nat.eqb_eq in HeqN1. subst n1.
+        rewrite Nat.eqb_neq in HeqN2.
+        rewrite double_update_indep in Heq4;
+        try symmetry; try assumption.
+        rewrite double_update in Heq4.
+        rewrite double_update_indep in Heq4;
+        try assumption.
+        subst Gamma'. subst Gamma''. subst Gamma'0.
+        rewrite double_update in H18.
+        rewrite double_update_indep in H18;
+        try assumption.
+        unfold well_typed in IHe1_3.
+        eexists (lub x x0 d_3). split.
+        --  apply more_specific_lub; try assumption.
+            eapply compatibility in H0. shelve.
+            eassumption.
+            eapply subst_preservation.
+            apply anyIn_cons_r; assumption.
+            apply Heq1. apply H1.
+            apply more_specific_refl.
+            Unshelve. destruct x;
+            try reflexivity; try inversion H0.
+        --  simpl. rewrite Nat.eqb_refl. simpl.
+            eapply Rule_CaseList;
+            try eassumption.
+            rewrite double_update_indep;
+            try eassumption.
+      + rewrite Nat.eqb_neq in HeqN1.
+        rewrite Nat.eqb_eq in HeqN2. subst n2.
+        subst Gamma'. subst Gamma''. subst Gamma'0.
+        rewrite double_update in Heq4.
+        rewrite double_update_indep in Heq4;
+        try symmetry; try assumption.
+        rewrite double_update_indep in H18;
+        try symmetry; try assumption.
+        rewrite double_update in H18.
+        unfold well_typed in IHe1_3.
+        eexists (lub x x0 d_3). split.
+        --  apply more_specific_lub; try assumption.
+            eapply compatibility in H0. shelve.
+            eassumption.
+            eapply subst_preservation.
+            apply anyIn_cons_r; assumption.
+            apply Heq1. apply H1.
+            apply more_specific_refl.
+            Unshelve. destruct x;
+            try reflexivity; try inversion H0.
+        --  simpl. rewrite Nat.eqb_refl.
+            rewrite <- Nat.eqb_neq in HeqN1.
+            rewrite HeqN1. simpl.
+            eapply Rule_CaseList;
+            try eassumption.
+            rewrite double_update_indep;
+            try eassumption.
+      + remember HeqN1 as HeqN1C.
+        remember HeqN2 as HeqN2C.
+        clear HeqHeqN1C. clear HeqHeqN2C.
+        rewrite Nat.eqb_neq in HeqN1.
+        rewrite Nat.eqb_neq in HeqN2.
+        rewrite (double_update_indep _ n0 _ n2) in Heq4.
+        rewrite (double_update_indep _ n0 _ n1) in Heq4.
+        subst Gamma'. subst Gamma''. subst Gamma'0.
+        rewrite (double_update_indep _ n0 _ n1) in H18.
+        rewrite (double_update_indep _ n0 _ n2) in H18.
+        edestruct IHe1_3 in H0_3.
+        apply anyIn_cons_r; try eassumption.
+        unfold well_typed. rewrite Heq4.
+        reflexivity. erewrite typeOf_unbound.
+        erewrite typeOf_unbound.
+        eassumption. eassumption. eassumption.
+        erewrite typeOf_unbound.
+        eassumption. eassumption. eassumption.
+        eassumption. shelve.
         eassumption. eassumption.
-        erewrite typeOf_unbound. erewrite typeOf_unbound.
-        apply H1. apply H1. assumption.
-        erewrite typeOf_unbound. eassumption. eassumption.
-        eassumption. eassumption.
-        erewrite <- update_compatible.
-        rewrite (double_update_indep _ n _ n1) in H12.
-        rewrite (double_update_indep _ n _ n2) in H12.
-        apply H12. assumption. assumption.
-        apply update_compatible. reflexivity. apply H3.
-        erewrite <- update_compatible with
-          (Gamma := mkCompatibleCtx (update Nat.eqb Rho n1 t0)).
-        erewrite <- update_compatible with
-          (Gamma := mkCompatibleCtx Rho).
-        eapply hasDType_unbound.
-        eapply hasDType_unbound.
-        apply H4. assumption. assumption. reflexivity. reflexivity.
-        destruct H6. destruct x.
-        ++  exists x0. split. assumption.
-            apply Rule_CaseDPair. assumption.
-            erewrite update_compatible. apply H7.
-            apply update_compatible. reflexivity.
-        ++  inversion H.
-        ++  inversion H.
+        eassumption.
+        apply hasDType_unbound. apply hasDType_unbound.
+        assumption. assumption. eassumption.
+        destruct H10. exists (lub x x0 x1). split.
+        * apply more_specific_lub; try assumption.
+          remember Heq1 as Heq1C. clear HeqHeq1C.
+          eapply compatibility in Heq1. shelve.
+          shelve. apply H12. Unshelve.
+          erewrite double_update_indep.
+          apply update_compatible; try assumption.
+          apply update_compatible; assumption.
+          assumption. shelve.
+          apply update_compatible; assumption.
+          Unshelve. eapply compatibility in H0. shelve.
+          eassumption.
+          eapply subst_preservation.
+          apply anyIn_cons_r; assumption.
+          apply Heq1C. apply H1.
+          Unshelve. destruct x;
+          try reflexivity; try inversion H0.
+        * simpl. rewrite HeqN1C.
+          rewrite HeqN2C. simpl.
+          eapply Rule_CaseList; eassumption.
+        * assumption.
+        * assumption.
+        * assumption.
+        * assumption.
   Qed.
 
   Lemma subst_lemma2 :
-    forall e1 e2 e3 Rho t1 t2 t3 n n3 d2' d3',
+    forall e1 e2 e3 Rho Gamma t1 t2 t3 d1 d2 d3 n n3 d2' d3',
     anyIn (freeVars e2) (n3::n::boundVars e1) = false ->
     anyIn (freeVars e3) (n3::n::boundVars e1) = false ->
     anyIn (freeVars e2) (boundVars e3) = false ->
@@ -2369,10 +2497,10 @@ Section Proofs.
     typeOf Rho e2 = Some t2 ->
     typeOf Rho e3 = Some t3 ->
     n <> n3 ->
-    let Gamma := mkCompatibleCtx Rho in
-    let d1 := mkCompatible t1 in
-    let d2 := mkCompatible t2 in
-    let d3 := mkCompatible t3 in
+    compatibleCtx Gamma Rho ->
+    compatible d1 t1 ->
+    compatible d2 t2 ->
+    compatible d3 t3 ->
     update Nat.eqb (update Nat.eqb Gamma n3 d3) n d2 |- e1 ::: d1 ->
     more_specific d2' d2 = true ->
     more_specific d3' d3 = true ->
@@ -2391,100 +2519,119 @@ Section Proofs.
     destruct (typeOf (update Nat.eqb (update Nat.eqb Rho n3 t3) n t2)
                    e1) eqn:Heq1;
     try inversion H2.
-    edestruct subst_lemma with (e1 := e1).
-    + apply anyIn_cons_r. apply H0. apply H13.
+    edestruct subst_lemma with (e1 := e1) (n := n3).
+    + apply anyIn_cons_r. apply H0. apply H17.
     + unfold well_typed.
       rewrite double_update_indep in Heq1.
       rewrite Heq1. reflexivity. symmetry. assumption.
     + erewrite typeOf_unbound. apply H4. apply H4. assumption.
-    + erewrite <- (update_compatible _ (Rho)).
-      erewrite double_update_indep.
-      apply H6. assumption. reflexivity.
-    + apply H8.
-    + erewrite <- update_compatible.
-      eapply (hasDType_unbound).
-      apply H10. assumption. reflexivity.
-    + destruct H15.
-      edestruct subst_lemma with (e1 := subst n3 e3 e1).
-      - apply anyIn_cons_r. apply any_in_subst. apply H. apply H13.
-        apply H1. apply H12.
+    + eapply (update_compatible _ (Rho)). eassumption.
+      eassumption.
+    + apply H9.
+    + rewrite double_update_indep in H10.
+      apply H10. symmetry. assumption.
+    + eassumption.
+    + apply hasDType_unbound; assumption.
+    + destruct H19.
+      edestruct subst_lemma with (e1 := subst n3 e3 e1) (n := n).
+      - apply anyIn_cons_r. apply any_in_subst. apply H. apply H17.
+        apply H1. apply H16.
       - unfold well_typed.
         erewrite subst_preservation. reflexivity.
-        apply anyIn_cons_r. apply H0. apply H13.
+        apply anyIn_cons_r. apply H0. apply H17.
         rewrite double_update_indep.
         rewrite Heq1. reflexivity. assumption.
         erewrite typeOf_unbound. assumption. eassumption. assumption.
       - assumption.
-      - erewrite update_compatible. apply H16. reflexivity.
-      - apply H7.
-      - apply H9.
-      - destruct H17. exists x0.
-        split. eapply more_specific_transitive. apply H17.
-        apply H15. apply H18.
+      - apply H6.
+      - apply H8.
+      - apply H20.
+      - eassumption.
+      - eassumption.
+      - destruct H21. exists x0.
+        split. eapply more_specific_transitive. apply H21.
+        apply H19. apply H22.
   Qed.
 
-  Lemma case_no_arrow : forall Rho e1 e2 d1 d2 b,
-    let Gamma := mkCompatibleCtx Rho in
+  Lemma case_no_arrow : forall Rho Gamma e1 e2 e3 e4 d1 d2 p,
+    compatibleCtx Gamma Rho ->
     (Gamma |- e1 ::: Arrow d1 d2 \/ Gamma |- e2 ::: Arrow d1 d2) ->
-    well_typed Rho (Case (Or e1 e2) b) ->
-    False.
+    (well_typed Rho (CaseL (Or e1 e2) e3 p e4) -> False) /\
+    (well_typed Rho (CaseB (Or e1 e2) e3 e4) -> False).
   Proof.
-    intros.
+    intros Rho Gamma e1 e2 e3 e4 d1 d2 p HC H.
+    split; intros H0.
+    --
     remember H0 as H0C. clear HeqH0C.
-    apply well_typed_Case in H0.
-    apply well_typed_Choice in H0.
-    destruct H0.
-    destruct H; destruct b.
-    - edestruct compatibility. reflexivity.
-      apply H0. apply H. destruct H2.
-      unfold well_typed in H0C.
-      unfold typeOf in H0C. fold typeOf in H0C.
-      destruct x; inversion H3.
-      rewrite H2 in H0C.
-      destruct (eqTypeS (Some (TArrow x1 x2))
-                        (typeOf Rho e2)) eqn:Heq;
+    destruct p.
+    apply well_typed_CaseL in H0.
+    destruct H0 as [H0A H0B].
+    apply well_typed_Choice in H0A.
+    destruct H0A. unfold well_typed in H0C.
+    unfold typeOf in H0C. fold typeOf in H0C.
+    destruct H.
+    - destruct (typeOf Rho e1) eqn:Heq1,
+               (typeOf Rho e2) eqn:Heq2;
+      try inversion H0C. simpl in H0C.
+      destruct (eqType t t0) eqn:Heq3;
+      try inversion H0C. destruct t; try inversion H0C.
+      apply eq_Type_eq in Heq3. subst.
+      eapply (compatibility e1 _ _ _ _ HC Heq1) in H.
+      inversion H.
+    - destruct (typeOf Rho e1) eqn:Heq1,
+               (typeOf Rho e2) eqn:Heq2;
+      try inversion H0C. simpl in H0C.
+      destruct (eqType t t0) eqn:Heq3;
+      try inversion H0C. destruct t; try inversion H0C.
+      simpl in H0C.
+      destruct (eqType t t1) eqn:Heq4;
       try inversion H0C.
-    - destruct p. edestruct compatibility. reflexivity.
-      apply H0. apply H. destruct H2.
-      unfold well_typed in H0C.
-      unfold typeOf in H0C. fold typeOf in H0C.
-      destruct x; inversion H3.
-      rewrite H2 in H0C.
-      destruct (eqTypeS (Some (TArrow x1 x2))
-                        (typeOf Rho e2)) eqn:Heq;
-      try inversion H0C.
-    - edestruct compatibility. reflexivity.
-      apply H1. apply H. destruct H2.
-      unfold well_typed in H0C.
-      unfold typeOf in H0C. fold typeOf in H0C.
-      destruct x; inversion H3.
-      rewrite H2 in H0C.
-      destruct (eqTypeS (typeOf Rho e1)
-                        (Some (TArrow x1 x2))) eqn:Heq;
-      try inversion H0C.
-      destruct (typeOf Rho e1) eqn:Heq2;
-      try inversion H0C.
-      destruct t; try inversion H0C. inversion Heq.
-    - destruct p. edestruct compatibility. reflexivity.
-      apply H1. apply H. destruct H2.
-      unfold well_typed in H0C.
-      unfold typeOf in H0C. fold typeOf in H0C.
-      destruct x; inversion H3.
-      rewrite H2 in H0C.
-      destruct (eqTypeS (typeOf Rho e1)
-                        (Some (TArrow x1 x2))) eqn:Heq;
-      try inversion H0C.
-      destruct (typeOf Rho e1) eqn:Heq2;
-      try inversion H0C.
-      destruct t; try inversion H0C. inversion Heq.
+      destruct (typeOf Rho e3) eqn:Heq5,
+               (typeOf (update Nat.eqb
+                       (update Nat.eqb Rho n2 (TList t1))
+                n1 t1) e4) eqn:Heq6;
+      try inversion H0C; simpl in H0C.
+      destruct (eqType t2 t3) eqn:Heq7;
+      try inversion H0C. apply eq_Type_eq in Heq3. subst.
+      eapply (compatibility e2 _ _ _ _ HC Heq2) in H.
+      inversion H.
+  --
+  remember H0 as H0C. clear HeqH0C.
+  destruct p.
+  apply well_typed_CaseB in H0.
+  destruct H0 as [H0A H0B].
+  apply well_typed_Choice in H0A.
+  destruct H0A. unfold well_typed in H0C.
+  unfold typeOf in H0C. fold typeOf in H0C.
+  destruct H.
+  - destruct (typeOf Rho e1) eqn:Heq1,
+             (typeOf Rho e2) eqn:Heq2;
+    try inversion H0C. simpl in H0C.
+    destruct (eqType t t0) eqn:Heq3;
+    try inversion H0C. destruct t; try inversion H0C.
+    apply eq_Type_eq in Heq3. subst.
+    eapply (compatibility e1 _ _ _ _ HC Heq1) in H.
+    inversion H.
+  - destruct (typeOf Rho e1) eqn:Heq1,
+             (typeOf Rho e2) eqn:Heq2;
+    try inversion H0C. simpl in H0C.
+    destruct (eqType t t0) eqn:Heq3;
+    try inversion H0C. destruct t; try inversion H0C.
+    destruct (typeOf Rho e3) eqn:Heq5,
+             (typeOf Rho e4) eqn:Heq6;
+    try inversion H0C; simpl in H0C.
+    destruct (eqType t t2) eqn:Heq7;
+    try inversion H0C. apply eq_Type_eq in Heq3. subst.
+    eapply (compatibility e2 _ _ _ _ HC Heq2) in H.
+    inversion H.
   Qed.
 
   (* Theorem preservation:
    Shows that if an expression e reduces to e', then the determinism type
    of e' is at least as specific as the determinism type of e.
    This is the core type safety property for the determinism type system. *)
-  Theorem preservation : forall Rho e e' t d,
-    let Gamma := mkCompatibleCtx Rho in
+  Theorem preservation : forall e e' Rho Gamma t d,
+    compatibleCtx Gamma Rho ->
     e ==> e' ->
     typeOf Rho e = Some t ->
     compatible d t ->
@@ -2492,82 +2639,49 @@ Section Proofs.
     exists d', more_specific d' d = true /\ compatible d' t
       /\ Gamma |- e' ::: d'.
   Proof.
-    intro Rho. intro e.
-    generalize dependent Rho.
-    induction e; intros Rho e' t0 d0 Gamma H HW HC H0; inversion H.
+    induction e; intros e' Rho Gamma t0 d0 HX H HW HC H0; inversion H.
+    * inversion H1.
+    * inversion H1.
     * inversion H1.
     * inversion H1.
     * inversion H1. inversion H0. subst.
       remember HW as HWC. clear HeqHWC.
       unfold typeOf in HW. fold typeOf in HW.
-      destruct (typeOf Rho e1) eqn:Heq1; try inversion HW.
-      destruct (typeOf Rho e2) eqn:Heq2;
+      destruct (typeOf Rho e2) eqn:Heq1;
+      try inversion HW; destruct t; try inversion HW.
+      destruct (typeOf Rho e1) eqn:Heq2;
       inversion HW; subst.
+      destruct (eqType t1 t) eqn:Heq3;
+      try inversion H6. subst.
+      apply eq_Type_eq in Heq3. subst t1.
       destruct (step e1) eqn:Heq.
       + remember Heq1 as Heq1C. clear HeqHeq1C.
-        destruct d1.
-        - edestruct (IHe1 Rho e t D). apply Single_Step.
-          apply Heq. eassumption. destruct t; try reflexivity.
-          edestruct compatibility. reflexivity. unfold well_typed.
-          rewrite Heq1. reflexivity. apply H7. destruct H2.
-          rewrite H2 in Heq1C. inversion Heq1C. subst.
-          inversion H4. apply H7.
-          apply (step_preservation e1 e Rho t Heq) in Heq1.
-          inversion H5. subst. destruct H2, H4, d2; subst.
-          --  destruct x; inversion H2; subst.
-              exists D. split. apply more_specific_refl.
-              split. reflexivity. eapply Rule_Pair. apply H6. apply H9. reflexivity.
-          --  exists ND. split. apply more_specific_ND. split. reflexivity.
-              eapply Rule_Pair. apply H6. apply H9.
-              destruct x; reflexivity.
-          --  exists ND. split. apply more_specific_ND. split. reflexivity.
-              eapply Rule_Pair. apply H6. apply H9.
-              destruct x; reflexivity.
-        - edestruct IHe1 with (d := ND). apply Single_Step.
-          apply Heq. eassumption. reflexivity. apply H7.
-          destruct H2, H4. inversion H5. subst.
-          eexists. split. apply more_specific_ND.
-          split. shelve. eapply Rule_Pair. apply H6. apply H9. reflexivity.
-          Unshelve. destruct x, d2; reflexivity.
-        - inversion H5. subst.
-          edestruct IHe1 with (d := Arrow d1_1 d1_2). apply Single_Step.
-          apply Heq. eassumption. edestruct compatibility. reflexivity.
-          unfold well_typed. rewrite Heq1. reflexivity. apply H7. destruct H2.
-          rewrite H2 in Heq1C. inversion Heq1C. subst. assumption. apply H7.
-          destruct H2, H4. inversion H5. subst.
-          eexists. split. apply more_specific_ND. split. shelve.
-          eapply Rule_Pair. apply H6. apply H9. reflexivity.
-          Unshelve. destruct x, d2; reflexivity.
-      + destruct (step e2) eqn:Heq3; inversion H5.
+        inversion H5. subst.
+        edestruct IHe1. eassumption.
+        apply Single_Step. apply Heq. eassumption. shelve.
+        apply H7. destruct H2, H8.
+        eexists. split. shelve. split. shelve.
+        eapply Rule_Cons. apply H10. apply H9.
+        reflexivity. Unshelve.
+        eapply compatibility. eassumption.
+        apply Heq2. eassumption.
+        destruct d1, d2, x; try reflexivity;
+        try inversion H8; try inversion H2.
+        destruct x, d2; reflexivity.
+      + destruct (step e2) eqn:Heq4; inversion H5.
+        subst.
         remember Heq2 as Heq2C. clear HeqHeq2C.
-        destruct d2.
-        - subst. edestruct (IHe2 Rho e t1 D). apply Single_Step. apply Heq3.
-          apply Heq2. destruct t1; try reflexivity.
-          edestruct compatibility. reflexivity. unfold well_typed.
-          rewrite Heq2. reflexivity. apply H9. destruct H2.
-          rewrite H2 in Heq2C. inversion Heq2C. subst.
-          inversion H4. apply H9. destruct H2, H4, d1; subst.
-          --  destruct x; try inversion H2.
-              exists D. split. apply more_specific_refl. split. reflexivity.
-              eapply Rule_Pair. apply H7. apply H6. reflexivity.
-          --  destruct x; try inversion H2. eexists. split. apply more_specific_ND.
-              split. shelve. eapply Rule_Pair. apply H7. apply H6. reflexivity.
-              Unshelve. reflexivity.
-          --  destruct x; try inversion H2. eexists. split. apply more_specific_ND.
-              split. shelve. eapply Rule_Pair. apply H7. apply H6. reflexivity.
-              Unshelve. reflexivity.
-        - edestruct IHe2 with (d := ND). apply Single_Step.
-          apply Heq3. eassumption. reflexivity. apply H9.
-          destruct H2, H6. eexists. split. destruct d1; apply more_specific_ND.
-          split. shelve. eapply Rule_Pair. apply H7. apply H8. reflexivity.
-          Unshelve. destruct x, d1; reflexivity.
-        - edestruct IHe2 with (d := Arrow d2_1 d2_2). apply Single_Step.
-          apply Heq3. eassumption. edestruct compatibility. reflexivity.
-          unfold well_typed. rewrite Heq2. reflexivity. apply H9. destruct H2.
-          rewrite H2 in Heq2C. inversion Heq2C. subst. assumption. apply H9.
-          destruct H2, H6. eexists. split. destruct d1; apply more_specific_ND. split. shelve.
-          eapply Rule_Pair. apply H7. apply H8. reflexivity.
-          Unshelve. destruct x, d1; reflexivity.
+        edestruct IHe2. eassumption.
+        apply Single_Step. apply Heq4. eassumption. shelve.
+        apply H9. destruct H2, H8.
+        eexists. split. shelve. split. shelve.
+        eapply Rule_Cons. apply H7. apply H10.
+        reflexivity. Unshelve.
+        eapply compatibility. eassumption.
+        apply Heq1. eassumption.
+        destruct d1, d2, x; try reflexivity;
+        try inversion H8; try inversion H2.
+        destruct x, d1; reflexivity.
     * inversion H1. subst.
       remember H0 as H0C. clear HeqH0C.
       remember HW as HWC. clear HeqHWC.
@@ -2580,22 +2694,28 @@ Section Proofs.
       destruct e1 eqn:Heq5.
       + simpl in H5. inversion H5.
       + inversion H5.
-      (* App Pair *)
-      + unfold well_typed in HWC.
-        unfold typeOf in HWC. fold typeOf in HWC.
-        destruct (typeOf Rho e3) eqn:Heq4;
-        try inversion HWC.
+      + inversion H5.
+      + inversion H5.
+      (* App Cons *)
+      + subst. simpl in Heq1.
         destruct (typeOf Rho e4) eqn:Heq6;
-        try inversion HWC; subst.
+        try inversion Heq1; subst.
+        destruct t; try inversion Heq1; subst.
+        destruct (typeOf Rho e3) eqn:Heq7;
+        try inversion Heq1; subst.
+        destruct (eqType t2 t) eqn:Heq8;
+        try inversion H9.
       (* App App *)
-      + destruct (step (App e3 e4)) eqn:Heq; inversion H5.
+      + destruct (step (App e3 e4)) eqn:Heq;
+        inversion H5.
         inversion H0; subst.
         - edestruct IHe1 with (d := d1).
+          eassumption.
           apply Single_Step. apply Heq. eassumption.
-          edestruct (compatibility (App e3 e4)). reflexivity.
-          unfold well_typed. rewrite Heq1. reflexivity. apply H11.
-          destruct H2. rewrite Heq1 in H2. inversion H2. subst.
-          assumption. apply H11. destruct H2, H7, x.
+          eapply (compatibility (App e3 e4)).
+          eassumption. assumption.
+          assumption. assumption.
+          destruct H2, H7, x.
           --  inversion H7.
           --  exists ND. split. apply more_specific_ND. split. reflexivity.
               eapply Rule_AppND. apply H8. apply H13.
@@ -2604,11 +2724,12 @@ Section Proofs.
               Unshelve. unfold decide. destruct (more_specific d2 x1).
               destruct H7. assumption. reflexivity.
         - edestruct IHe1 with (d := (Arrow d1 d2)).
+          eassumption.
           apply Single_Step. apply Heq. eassumption.
-          edestruct (compatibility (App e3 e4)). reflexivity.
-          unfold well_typed. rewrite Heq1. reflexivity. apply H10.
-          destruct H2. rewrite Heq1 in H2. inversion H2. subst.
-          assumption. apply H10. destruct H2, H7, x.
+          eapply (compatibility (App e3 e4)).
+          eassumption. assumption.
+          assumption. assumption.
+          destruct H2, H7, x.
           --  inversion H7.
           --  inversion H2.
           --  simpl in H2. apply (andb_true_iff) in H2. destruct H2.
@@ -2639,25 +2760,31 @@ Section Proofs.
         destruct (eqType t2 t4) eqn:Heq8; try inversion HWC.
         apply eq_Type_eq in Heq8. subst. inversion H0.
         - inversion Heq3. inversion H12; subst.
-          edestruct (compatibility (Abs n t1 e)). reflexivity.
-          unfold well_typed. rewrite Heq1. reflexivity.
-          apply H12. destruct H2. rewrite Heq1 in H2. inversion H2. subst.
-          inversion H7. specialize (step_preservation _ _ _ _ H1 HWC2). intros.
-          edestruct (compatibility e2). reflexivity.
-          unfold well_typed. rewrite Heq6. reflexivity. eassumption.
-          destruct H16. rewrite Heq6 in H16. inversion H16; subst.
-          edestruct subst_lemma.
-          eassumption. unfold well_typed.
-          rewrite Heq4. reflexivity. assumption. apply H22. shelve.
-          apply H14. destruct H18. eexists. split. apply more_specific_ND.
-          split. shelve. apply H19. Unshelve.
-          give_up. give_up.
-        - inversion H11; subst. edestruct subst_lemma.
-          eassumption. unfold well_typed. rewrite Heq4. reflexivity.
-          apply Heq6. shelve. shelve. apply H13.
-          destruct H2. eexists. split.
-          shelve. split. shelve. apply H7. Unshelve.
-          give_up. give_up. give_up. give_up. give_up.
+          remember HX as HXC. clear HeqHXC.
+          eapply (compatibility (Abs n t1 e)) in HX. shelve.
+          simpl. rewrite Heq4. reflexivity. apply H12.
+          Unshelve. simpl in HX. destruct HX.
+          edestruct (completeness (subst n e2 e)).
+          eassumption. eapply subst_preservation.
+          eassumption. apply Heq4. apply Heq6.
+          destruct H11. exists x.
+          split. apply more_specific_ND.
+          split. apply H13. apply H11.
+        - inversion H11; subst. unfold decide in *.
+          destruct (more_specific d3 d1) eqn:Heq5.
+          --  edestruct subst_lemma. eassumption.
+              unfold well_typed. rewrite Heq4. reflexivity.
+              apply Heq6. eassumption. apply H19. apply H23. apply Heq5. apply H13.
+              destruct H2.
+              eexists. split. apply H2.
+              split. shelve. apply H7. Unshelve.
+              eapply compatibility. eassumption.
+              eapply subst_preservation. eassumption.
+              apply Heq4. apply Heq6. apply H7.
+          --  edestruct completeness. eassumption. shelve.
+              destruct H2. eexists. split.
+              apply more_specific_ND. split. apply H7. apply H2.
+              Unshelve. eapply subst_preservation; eassumption.
       (* App Or *)
       + destruct d0.
         - inversion H0; inversion H6. inversion H9.
@@ -2674,49 +2801,71 @@ Section Proofs.
           shelve. assumption. Unshelve. unfold typeOf in HWC.
           fold typeOf in HWC. rewrite Heq6, Heq7, Heq3, eqTypeS_refl in HWC.
           rewrite eqType_refl in HWC.
-          edestruct (completeness (App e3 e2)). reflexivity.
-          unfold well_typed. unfold typeOf. fold typeOf.
-          rewrite Heq6, Heq3, eqType_refl. reflexivity.
-          edestruct (completeness (App e4 e2)). reflexivity.
-          unfold well_typed. unfold typeOf. fold typeOf.
-          rewrite Heq7, Heq3, eqType_refl. reflexivity.
-          eapply Rule_Choice. eassumption. eassumption.
+          edestruct (completeness (App e3 e2)). eassumption.
+          simpl. rewrite Heq6, Heq3, eqType_refl. reflexivity.
+          destruct H2. edestruct (completeness (App e4 e2)). eassumption.
+          simpl. rewrite Heq7, Heq3, eqType_refl. reflexivity.
+          destruct H8. eapply Rule_Choice. eassumption. eassumption.
         - inversion H0; inversion H6. inversion H9.
       (* App Case *)
-      + destruct (step (Case e b)) eqn:Heq; inversion H5; subst.
+      + destruct (step (CaseB e3 e4 e5)) eqn:Heq; inversion H5; subst.
         inversion H0; subst.
-        - edestruct (compatibility (Case e b)). reflexivity.
-          unfold well_typed. rewrite Heq1. reflexivity. apply H9.
-          destruct H2. rewrite Heq1 in H2. inversion H2. subst.
-          edestruct IHe1. apply Single_Step. apply Heq. eassumption.
-          eassumption. apply H9. destruct H8, H10, x.
-          --  inversion H10.
-          --  exists ND. split. apply more_specific_ND.
-              split. reflexivity.
-              eapply Rule_AppND. apply H12. apply H11.
-          --  eexists. split. apply more_specific_ND.
-              split. shelve.
-              eapply Rule_AppFun. apply H12. apply H11. reflexivity.
-              Unshelve. unfold decide.
-              destruct (more_specific d2 x1).
-              simpl in H10. destruct H10. assumption. reflexivity.
-        - edestruct (compatibility (Case e b)). reflexivity.
-          unfold well_typed. rewrite Heq1. reflexivity. apply H8.
-          destruct H2. rewrite Heq1 in H2. inversion H2. subst.
-          edestruct IHe1. apply Single_Step. apply Heq. eassumption.
-          eassumption. apply H8. destruct H9, H11, x; inversion H11;
-          inversion H9. apply andb_true_iff in H16. destruct H16.
-          unfold decide. rewrite H15. rewrite H16. simpl.
-          destruct (more_specific d3 d1) eqn:Heq2.
-          --  rewrite less_specific_more_specific in H15.
-              eapply more_specific_transitive in H15.
+        - edestruct IHe1. eassumption. apply Single_Step. apply Heq.
+          rewrite Heq1. reflexivity. eapply compatibility.
+          eassumption. apply Heq1. eassumption. apply H9.
+          destruct H2, H7.
+          exists ND. split. apply more_specific_ND.
+          split. reflexivity.
+          eapply Rule_AppND. apply H8. apply H11.
+        - edestruct IHe1. eassumption. apply Single_Step.
+          apply Heq. rewrite Heq1. reflexivity. eapply compatibility.
+          eassumption. apply Heq1. eassumption. apply H8.
+          destruct H2, H7, x.
+          --  inversion H7.
+          --  inversion H2.
+          --  simpl in H2. apply (andb_true_iff) in H2.
+              destruct H2. simpl in H7. destruct H7.
+              rewrite <- more_specific_less_specific in H2.
               eexists. split. shelve. split. shelve.
-              eapply Rule_AppFun. apply H12. apply H10.
-              reflexivity. apply Heq2. Unshelve.
-              unfold decide. rewrite H15. assumption.
-              unfold decide. rewrite H15. assumption.
-          --  eexists. split. apply more_specific_ND.
-              split. shelve. eapply Rule_AppFun. apply H12. apply H10. reflexivity. Unshelve.
+              eapply Rule_AppFun. apply H9. apply H10.
+              reflexivity. Unshelve.
+              unfold decide.
+              destruct (more_specific d3 x1) eqn:M1,
+                       (more_specific d3 d1) eqn:M2.
+              assumption. apply more_specific_ND.
+              apply more_specific_transitive with (d1:=d3) (d2:=d1) (d3:=x1) in M2.
+              rewrite M1 in M2. inversion M2.
+              assumption. apply more_specific_ND.
+              unfold decide. destruct (more_specific d3 x1).
+              assumption. reflexivity.
+      + destruct (step (CaseL e3 e4 p e5)) eqn:Heq; inversion H5; subst.
+        inversion H0; subst.
+        - edestruct IHe1. eassumption. apply Single_Step. apply Heq.
+          rewrite Heq1. reflexivity. eapply compatibility.
+          eassumption. apply Heq1. eassumption. apply H9.
+          destruct H2, H7.
+          exists ND. split. apply more_specific_ND.
+          split. reflexivity.
+          eapply Rule_AppND. apply H8. apply H11.
+        - edestruct IHe1. eassumption. apply Single_Step.
+          apply Heq. rewrite Heq1. reflexivity. eapply compatibility.
+          eassumption. apply Heq1. eassumption. apply H8.
+          destruct H2, H7, x.
+          --  inversion H7.
+          --  inversion H2.
+          --  simpl in H2. apply (andb_true_iff) in H2.
+              destruct H2. simpl in H7. destruct H7.
+              rewrite <- more_specific_less_specific in H2.
+              eexists. split. shelve. split. shelve.
+              eapply Rule_AppFun. apply H9. apply H10.
+              reflexivity. Unshelve.
+              unfold decide.
+              destruct (more_specific d3 x1) eqn:M1,
+                       (more_specific d3 d1) eqn:M2.
+              assumption. apply more_specific_ND.
+              apply more_specific_transitive with (d1:=d3) (d2:=d1) (d3:=x1) in M2.
+              rewrite M1 in M2. inversion M2.
+              assumption. apply more_specific_ND.
               unfold decide. destruct (more_specific d3 x1).
               assumption. reflexivity.
     * inversion H1.
@@ -2729,150 +2878,183 @@ Section Proofs.
       apply eq_Type_eq in Heq2. subst.
       destruct (step e1) eqn:Heq3.
       + inversion H5. subst.
-        edestruct IHe1. apply Single_Step. eassumption.
+        edestruct IHe1. eassumption. apply Single_Step. eassumption.
         eassumption. shelve. eassumption.
         destruct H2, H4. exists ND. split. apply more_specific_refl.
         split. reflexivity. eapply Rule_Choice; eassumption.
-        Unshelve. edestruct (compatibility e1). reflexivity.
-        unfold well_typed. rewrite Heq1. reflexivity.
-        eassumption. destruct H2.
-        rewrite Heq1 in H2. inversion H2. subst. assumption.
+        Unshelve. eapply (compatibility e1). eassumption.
+        apply Heq1. eassumption.
       + destruct (step e2) eqn:Heq2; inversion H5. subst.
-        edestruct IHe2. apply Single_Step. eassumption.
+        edestruct IHe2. eassumption. apply Single_Step. eassumption.
         eassumption. shelve. eassumption.
         destruct H2, H4. exists ND. split. apply more_specific_refl.
         split. reflexivity. eapply Rule_Choice; eassumption.
-        Unshelve. edestruct (compatibility e2). reflexivity.
-        unfold well_typed. rewrite Heq11. reflexivity.
-        eassumption. destruct H2.
-        rewrite Heq11 in H2. inversion H2. subst. assumption.
+        Unshelve. eapply (compatibility e2). eassumption.
+        apply Heq11. eassumption.
     (* Case *)
-    * inversion H1. destruct e eqn:Heq1; inversion H5.
-      + destruct b; inversion H5; subst. inversion H0; subst.
-        - inversion H7. inversion H2.
-        - exists d0. split. apply more_specific_refl.
-          split. assumption. assumption.
-      + destruct b; inversion H5; subst. destruct p.
-        destruct (anyIn (freeVars e1_1 ++ freeVars e1_2)
-                        (n1 :: n2 :: boundVars e1)) eqn:Heq1;
-        inversion H5.
-        destruct (anyIn (freeVars e1_2) (boundVars e1_1)) eqn:Heq2;
-        inversion H5.
-        apply anyIn_concat2 in Heq1. destruct Heq1 as [HH1 HH2].
-        unfold typeOf in HW. fold typeOf in HW.
-        destruct (typeOf Rho e1_1) eqn:Heq1; try discriminate.
-        destruct (typeOf Rho e1_2) eqn:Heq3; try discriminate.
-        destruct (eqType t1 t) eqn:Heq4; try discriminate.
-        destruct (eqType t2 t3) eqn:Heq5; try discriminate.
-        apply eq_Type_eq in Heq4. apply eq_Type_eq in Heq5. subst.
-        simpl in HW.
-        inversion H0; subst.
-        - (* do it via completeness instead*)
-          inversion H17. subst.
-          edestruct (compatibility e1_1). reflexivity.
-          unfold well_typed. rewrite Heq1. reflexivity.
-          apply H9. destruct H4. rewrite Heq1 in H4. inversion H4. subst.
-          edestruct (compatibility e1_2). reflexivity.
-          unfold well_typed. rewrite Heq3. reflexivity.
-          apply H12. destruct H10. rewrite Heq3 in H10. inversion H10. subst.
-          edestruct subst_lemma2.
-          apply HH2. apply HH1. assumption.
-          unfold well_typed. rewrite HW. reflexivity.
-          assumption. assumption.  symmetry. assumption.
-          subst Gamma'. subst Gamma''. shelve. shelve. shelve.
-          apply H12. apply H9. destruct H16. eexists. split.
-          apply more_specific_ND. split. shelve. apply H19.
-          Unshelve. shelve. shelve. give_up. give_up. give_up.
-        - inversion H17. destruct d1, d2; inversion H15. subst.
-          edestruct subst_lemma2.
-          apply HH2. apply HH1. assumption.
-          unfold well_typed. rewrite HW. reflexivity.
-          assumption. assumption. symmetry. assumption.
-          subst Gamma'. subst Gamma''. shelve. shelve. shelve.
-          apply H12. apply H9.
-          destruct H4. exists x. split. shelve.
-          split. shelve. apply H8.
-          Unshelve. give_up. give_up. give_up. give_up.
-          give_up. give_up. give_up. give_up.
-      + subst. inversion H0; try inversion H6; try inversion H7; subst.
-        - remember HW as HWC. clear HeqHWC.
-          unfold typeOf in HW. fold typeOf in HW.
-          destruct (typeOf Rho e1_1) eqn:Heq1,
-                   (typeOf Rho e1_2) eqn:Heq2;
-          try discriminate. simpl in HW.
-          destruct (eqType t t1) eqn:Heq3; try discriminate.
-          apply eq_Type_eq in Heq3. subst.
-          destruct t1; try discriminate.
-          eexists ND. split. apply more_specific_refl.
-          split. reflexivity.
-          destruct d1; destruct d2.
-          --  eapply Rule_Choice; eapply Rule_CaseDUnit;
-              eassumption.
-          --  eapply Rule_Choice. eapply Rule_CaseDUnit.
-              eassumption. eassumption.
-              eapply Rule_CaseNDUnit; eassumption.
-          --  edestruct case_no_arrow.
-              right. apply H13. unfold well_typed.
-              rewrite HWC. reflexivity.
-          --  eapply Rule_Choice. eapply Rule_CaseNDUnit.
-              eassumption. eassumption.
-              eapply Rule_CaseDUnit; eassumption.
-          --  eapply Rule_Choice; eapply Rule_CaseNDUnit;
-              eassumption.
-          --  edestruct case_no_arrow.
-              right. apply H13. unfold well_typed.
-              rewrite HWC. reflexivity.
-          --  edestruct case_no_arrow.
-              left. apply H12. unfold well_typed.
-              rewrite HWC. reflexivity.
-          --  edestruct case_no_arrow.
-              left. apply H12. unfold well_typed.
-              rewrite HWC. reflexivity.
-          --  edestruct case_no_arrow.
-              right. apply H13. unfold well_typed.
-              rewrite HWC. reflexivity.
-        - remember HW as HWC. clear HeqHWC.
-          unfold typeOf in HW. fold typeOf in HW.
-          destruct (typeOf Rho e1_1) eqn:Heq1,
-                   (typeOf Rho e1_2) eqn:Heq2;
-          try discriminate. simpl in HW.
-          destruct (eqType t t3) eqn:Heq3; try discriminate.
-          apply eq_Type_eq in Heq3. subst.
-          destruct t3; try discriminate.
-          eexists ND. split. apply more_specific_refl.
-          split. reflexivity.
-          destruct d1, d2.
-          --  eapply Rule_Choice; eapply Rule_CaseDPair;
-              eassumption.
-          --  eapply Rule_Choice. eapply Rule_CaseDPair.
-              eassumption. eassumption.
-              eapply Rule_CaseNDPair; eassumption.
-          --  edestruct case_no_arrow.
-              right. apply H15. unfold well_typed.
-              rewrite HWC. reflexivity.
-          --  eapply Rule_Choice. eapply Rule_CaseNDPair.
-              eassumption. eassumption.
-              eapply Rule_CaseDPair; eassumption.
-          --  eapply Rule_Choice; eapply Rule_CaseNDPair;
-              eassumption.
-          --  edestruct case_no_arrow.
-              right. apply H15. unfold well_typed.
-              rewrite HWC. reflexivity.
-          --  edestruct case_no_arrow.
-              left. apply H14. unfold well_typed.
-              rewrite HWC. reflexivity.
-          --  edestruct case_no_arrow.
-              left. apply H14. unfold well_typed.
-              rewrite HWC. reflexivity.
-          --  edestruct case_no_arrow.
-              right. apply H15. unfold well_typed.
-              rewrite HWC. reflexivity.
-  Admitted.
+    * inversion H1. inversion H0. subst.
+      remember HW as HWC. clear HeqHWC.
+      unfold typeOf in HW. fold typeOf in HW.
+      destruct (typeOf Rho e1) eqn:Heq1; try inversion HW.
+      destruct t eqn:Heq2; try inversion HW.
+      destruct (typeOf Rho e2) eqn:Heq3; try inversion HW.
+      destruct (typeOf Rho e3) eqn:Heq5; try inversion HW.
+      destruct (eqType t1 t2) eqn:Heq4; try inversion HW.
+      apply eq_Type_eq in Heq4. inversion HW. subst.
+      destruct e1; inversion H5; subst.
+      + eexists. split. shelve. split. shelve. apply H12.
+        Unshelve. apply more_specific_lub''.
+        eapply compatibility. apply HX. apply Heq5.
+        apply H12.
+      + eexists. split. shelve. split. shelve. apply H11.
+        Unshelve. apply more_specific_lub'.
+        eapply compatibility. apply HX. apply Heq3.
+        apply H11.
+      + inversion H9. subst. exists ND. split.
+        destruct d2, d3; reflexivity.
+        split. reflexivity. simpl in Heq1.
+        destruct (typeOf Rho e1_1) eqn:Heq6;
+        try inversion Heq1; subst;
+        destruct (typeOf Rho e1_2) eqn:Heq7;
+        try inversion Heq1; subst.
+        destruct (eqType t t1) eqn:Heq8;
+        try inversion H8; subst.
+        apply eq_Type_eq in Heq8. subst.
+        edestruct (completeness (CaseB e1_2 e2 e3)).
+        eassumption. unfold well_typed. simpl.
+        rewrite Heq7, Heq3, Heq5. rewrite eqType_refl. reflexivity.
+        destruct H2. edestruct (completeness (CaseB e1_1 e2 e3)).
+        eassumption. unfold well_typed. simpl.
+        rewrite Heq6, Heq3, Heq5. rewrite eqType_refl. reflexivity.
+        destruct H17. eapply Rule_Choice; eapply Rule_CaseBool; eassumption.
+    * destruct p. inversion H1. inversion H0. subst.
+      remember HW as HWC. clear HeqHWC.
+      unfold typeOf in HW. fold typeOf in HW.
+      destruct (typeOf Rho e1) eqn:Heq1; try inversion HW;
+      destruct (eqType t (TList t1)) eqn:Heq2; try inversion H3.
+      apply eq_Type_eq in Heq2. subst.
+      destruct (typeOf Rho e2) eqn:Heq3,
+               (typeOf (update Nat.eqb (update Nat.eqb Rho n2 (TList t1)) n1 t1) e3) eqn:Heq4;
+      simpl in H3; try discriminate; subst.
+      destruct (eqType t t2) eqn:Heq5; try inversion H3.
+      apply eq_Type_eq in Heq5. subst.
+      destruct e1; inversion H5; subst.
+      + eexists. split. shelve. split. shelve. apply H19.
+        Unshelve. apply more_specific_lub'.
+        eapply compatibility. apply HX. apply Heq3.
+        apply H19.
+      + destruct (anyIn (freeVars e1_1 ++ freeVars e1_2) (n1 :: n2 :: boundVars e3)) eqn:Heq6;
+        try discriminate. destruct (anyIn (freeVars e1_2) (boundVars e1_1)) eqn:Heq7;
+        try discriminate. inversion H7. subst.
+        apply anyIn_concat2 in Heq6. destruct Heq6.
+        simpl in Heq1.
+        destruct (typeOf Rho e1_2) eqn:Heq8; try discriminate.
+        destruct t; try discriminate.
+        destruct (typeOf Rho e1_1) eqn:Heq9; try discriminate.
+        simpl in Heq1.
+        destruct (eqType t2 t) eqn:Heq10; try discriminate.
+        apply eq_Type_eq in Heq10. subst.
+        inversion Heq1. inversion H16. subst. subst Gamma'. subst Gamma''.
+        specialize (compatibility _ _ _ _ _ HX Heq8 H21) as H22.
+        specialize (compatibility _ _ _ _ _ HX Heq9 H13) as H23.
+        specialize (compatibility _ _ _ _ _ HX Heq3 H19) as H24.
+        rewrite double_update_indep in Heq4; try symmetry; try assumption.
+        specialize (update_update_compatible _ _ n1 n2 _ _ _ _ HX H17 H18) as HXC.
+        specialize (compatibility _ _ _ _ _ HXC Heq4 H20)  as H25.
+        destruct (more_specific d3 d2) eqn:Heq11,
+                 (more_specific d0 d1) eqn:Heq12.
+        ---
+        edestruct subst_lemma2. apply H8. apply H2.
+        apply Heq7. unfold well_typed.
+        rewrite Heq4. reflexivity.
+        apply Heq8. apply Heq9. symmetry. assumption. eassumption.
+        apply H25. apply H18. apply H17.
+        apply H20. apply Heq11. apply Heq12. apply H21. apply H13.
+        destruct H10. exists x. split.
+        **  destruct d0.
+            --  destruct d3.
+                ++ destruct d_2, d_3; unfold lub, lub2; simpl; try apply more_specific_ND.
+                  apply H10.
+                ++ destruct d_2, d_3; simpl; apply more_specific_ND.
+                ++ destruct d_2, d_3; simpl; apply more_specific_ND.
+            -- destruct d_2, d_3; simpl; apply more_specific_ND.
+            -- destruct d_2, d_3; simpl; apply more_specific_ND.
+        **  split. eapply compatibility. apply HX.
+            eapply subst_preservation2. apply H8. apply H2.
+            apply Heq7. symmetry. assumption. rewrite Heq4.
+            reflexivity. assumption. apply Heq9. apply H11.
+            apply H11.
+        --- destruct t1, d0, d1; try inversion Heq12;
+            try inversion H17; try inversion H23.
+            +++ edestruct completeness. apply HX.
+                eapply subst_preservation2.
+                apply H8. apply H2. assumption. symmetry. assumption.
+                rewrite Heq4. reflexivity. apply Heq8. apply Heq9.
+                destruct H10. exists x.
+                split. destruct d_2, d_3; apply more_specific_ND.
+                split. assumption. assumption.
+            +++ edestruct completeness. apply HX.
+                eapply subst_preservation2.
+                apply H8. apply H2. assumption. symmetry. assumption.
+                rewrite Heq4. reflexivity. apply Heq8. apply Heq9.
+                destruct H10. exists x.
+                split. destruct d_2, d_3; apply more_specific_ND.
+                split. assumption. assumption.
+            +++ edestruct completeness. apply HX.
+                eapply subst_preservation2.
+                apply H8. apply H2. assumption. symmetry. assumption.
+                rewrite Heq4. reflexivity. apply Heq8. apply Heq9.
+                destruct H12. exists x.
+                split. destruct d_2, d_3; apply more_specific_ND.
+                split. assumption. assumption.
+            +++ edestruct completeness. apply HX.
+                eapply subst_preservation2.
+                apply H8. apply H2. assumption. symmetry. assumption.
+                rewrite Heq4. reflexivity. apply Heq8. apply Heq9.
+                destruct H27. exists x.
+                split. destruct d_2, d_3; apply more_specific_ND.
+                split. assumption. assumption.
+        --- destruct d3, d2; try inversion Heq11;
+            try inversion H22; try inversion H18.
+            edestruct completeness. apply HX.
+            eapply subst_preservation2.
+            apply H8. apply H2. assumption. symmetry. assumption.
+            rewrite Heq4. reflexivity. apply Heq8. apply Heq9.
+            destruct H10. exists x.
+            split. destruct d0, d_2, d_3; apply more_specific_ND.
+            split. assumption. assumption.
+        --- destruct d3, d2; try inversion Heq11;
+            try inversion H22; try inversion H18.
+            edestruct completeness. apply HX.
+            eapply subst_preservation2.
+            apply H8. apply H2. assumption. symmetry. assumption.
+            rewrite Heq4. reflexivity. apply Heq8. apply Heq9.
+            destruct H10. exists x.
+            split. destruct d0, d_2, d_3; apply more_specific_ND.
+            split. assumption. assumption.
+      + inversion H16. subst. exists ND. split.
+        destruct d_2, d_3; reflexivity.
+        split. reflexivity. simpl in Heq1.
+        destruct (typeOf Rho e1_1) eqn:Heq6;
+        try inversion Heq1; subst;
+        destruct (typeOf Rho e1_2) eqn:Heq7;
+        try inversion Heq1; subst.
+        destruct (eqType t t2) eqn:Heq8;
+        try inversion H8; subst.
+        apply eq_Type_eq in Heq8. subst.
+        edestruct (completeness (CaseL e1_2 e2 (Pat n1 t1 n2 n) e3)).
+        eassumption. unfold well_typed. simpl.
+        rewrite Heq7, Heq3, Heq4. rewrite eqTypeS_refl. rewrite eqTypeS_refl. reflexivity.
+        destruct H2. edestruct (completeness (CaseL e1_1 e2 (Pat n1 t1 n2 n) e3)).
+        eassumption. unfold well_typed. simpl.
+        rewrite Heq6, Heq3, Heq4. rewrite eqTypeS_refl. rewrite eqTypeS_refl. reflexivity.
+        destruct H13. eapply Rule_Choice; eapply Rule_CaseList; eassumption.
+  Qed.
 
   Theorem preservation_multi : forall e e' t,
     e ==>* e' ->
-    forall Rho d,
-    let Gamma := mkCompatibleCtx Rho in
+    forall Rho Gamma d,
+    compatibleCtx Gamma Rho ->
     typeOf Rho e = Some t ->
     compatible d t ->
     Gamma |- e ::: d ->
@@ -2884,12 +3066,12 @@ Section Proofs.
     * exists d. split. apply more_specific_refl.
       split; assumption.
     * remember H as HC. clear HeqHC. inversion HC.
-      remember H1 as H1C. clear HeqH1C.
-      eapply (step_preservation _ _ _ _ H4) in H1.
-      apply (preservation Rho e1 e2 t d) in H; try assumption.
-      destruct H, H, H5, H7.
-      destruct (IHmulti_step_rel Rho x).
-      assumption. assumption. apply H7. destruct H8, H9.
+      remember H2 as H2C. clear HeqH2C.
+      eapply (step_preservation _ _ _ _ H5) in H2.
+      apply (preservation e1 e2 Rho Gamma t d) in H; try assumption.
+      destruct H, H, H5, H8.
+      destruct (IHmulti_step_rel Rho Gamma x).
+      assumption. assumption. apply H5. apply H8. destruct H9, H10.
       exists x0. split. eapply more_specific_transitive.
       eassumption. eassumption. split; assumption.
   Qed.
@@ -2898,8 +3080,8 @@ Section Proofs.
    The main theorem showing that if an expression e has deterministic type D,
    then any expression e' that e reduces to will not be a non-deterministic choice.
    This validates that the determinism type system correctly tracks non-determinism. *)
-  Theorem soundness : forall Rho e e' t,
-    let Gamma := mkCompatibleCtx Rho in
+  Theorem soundness : forall Rho Gamma e e' t,
+    compatibleCtx Gamma Rho ->
     typeOf Rho e = Some t ->
     Gamma |- e ::: D ->
     compatible D t ->
@@ -2909,11 +3091,13 @@ Section Proofs.
     intros. unfold well_typed in H. destruct (typeOf Rho e) eqn:Heq;
     try inversion H. edestruct (preservation_multi e e') in H0.
     - assumption.
-    - rewrite Heq. reflexivity.
-    - inversion H; apply H1.
+    - eassumption.
+    - apply Heq.
+    - inversion H0; subst. apply H2.
     - assumption.
-    - destruct H3. destruct H5. apply more_specific_D in H3.
+    - destruct H4. destruct H5. apply more_specific_D in H4.
       subst. destruct e'; try reflexivity; try inversion H6.
+    - inversion H0.
   Qed.
 
 End Proofs.
